fix more lemmas

viper-total-heaps/ViperBoogieEndToEnd.thy
@@ -2,7 +2,7 @@ theory ViperBoogieEndToEnd
 imports StmtRel
 begin
 
-text \<open>Accesses to old expressions are represented via labeled old expressions with label \<^const>\<open>old_label\<close>.\<close>  
+text \<open>Accesses to old expressions are represented via labeled old expressions with label \<^const>\<open>old_label\<close>.\<close>
 
 lemma valid_configuration_not_failure:
   assumes "valid_configuration A \<Lambda> \<Gamma> \<Omega> posts bb cont state"
@@ -11,11 +11,11 @@ lemma valid_configuration_not_failure:
   unfolding valid_configuration_def
   by simp
 
-type_synonym ('a,'m) proc_body_satisfies_spec_ty = 
+type_synonym ('a,'m) proc_body_satisfies_spec_ty =
    "'a absval_ty_fun \<Rightarrow> 'm proc_context \<Rightarrow> var_context \<Rightarrow> 'a fun_interp \<Rightarrow> rtype_env \<Rightarrow> expr list \<Rightarrow> expr list \<Rightarrow> ast \<Rightarrow> 'a nstate \<Rightarrow> bool"
 
-abbreviation state_rel_well_def_same where 
-  "state_rel_well_def_same ctxt Pr StateCons TyRep Tr AuxPred w ns \<equiv> 
+abbreviation state_rel_well_def_same where
+  "state_rel_well_def_same ctxt Pr StateCons TyRep Tr AuxPred w ns \<equiv>
        state_rel Pr StateCons TyRep Tr AuxPred ctxt w w ns"
 
 text \<open>The following lemma will not hold once we track old states.\<close>
@@ -23,9 +23,9 @@ text \<open>The following lemma will not hold once we track old states.\<close>
 lemma state_rel_well_def_same_old_state:
   assumes "state_rel_well_def_same ctxt Pr StateCons TyRep Tr AuxPred w ns" and
           "wf_total_consistency ctxt_vpr StateCons StateCons_t"
-          "\<And>l \<phi>. t l = Some \<phi> \<Longrightarrow> StateCons_t \<phi>" 
+          "\<And>l \<phi>. t l = Some \<phi> \<Longrightarrow> StateCons_t \<phi>"
   shows "state_rel_well_def_same ctxt Pr StateCons TyRep Tr AuxPred (update_trace_total w t) ns"
-  unfolding state_rel_def state_rel0_def 
+  unfolding state_rel_def state_rel0_def
   using state_rel_trace_independent
   oops
 (*
@@ -52,16 +52,16 @@ lemma magic_stays_red_bigblock_multi:
    assumes "red_bigblock_multi A M \<Lambda> \<Gamma> \<Omega> ast \<gamma> \<gamma>'" and
       "snd (snd \<gamma>) = Magic"
     shows "snd (snd \<gamma>') = Magic"
-  using assms 
+  using assms
   apply induction
    apply simp
   using magic_stays_red_bigblock
-  by blast  
+  by blast
 
 inductive_cases RedSimpleCmdsCons_case: "A,M,\<Lambda>,\<Gamma>,\<Omega>,T \<turnstile> \<langle>((BigBlock bb_name (c#cs) str_cmd tr_cmd), cont0, Normal n_s)\<rangle> \<longrightarrow> y"
 
 lemma red_bigblock_multi_simple_cmds_cons_failure:
-  assumes 
+  assumes
           RedMulti: "red_bigblock_multi A M \<Lambda> \<Gamma> \<Omega> ast \<gamma> \<gamma>'" and
                "\<gamma> = (BigBlock name cs str tr, cont, s')" and
           RedSingleCmd: "A, M, \<Lambda>, \<Gamma>, \<Omega> \<turnstile> \<langle>c, s\<rangle> \<rightarrow> s'" and
@@ -80,7 +80,7 @@ proof (cases s')
     by blast
 
   from this
-  obtain s'' where "A, M, \<Lambda>, \<Gamma>, \<Omega> \<turnstile> \<langle>cs, Normal ns\<rangle> [\<rightarrow>] s''" and 
+  obtain s'' where "A, M, \<Lambda>, \<Gamma>, \<Omega> \<turnstile> \<langle>cs, Normal ns\<rangle> [\<rightarrow>] s''" and
                    RedMultiEmptySimpleCmds: "red_bigblock_multi A M \<Lambda> \<Gamma> \<Omega> ast (BigBlock name [] str tr, cont, s'') \<gamma>'"
   proof -
     assume *: "(\<And>s''. A,M,\<Lambda>,\<Gamma>,\<Omega> \<turnstile> \<langle>cs,Normal ns\<rangle> [\<rightarrow>] s'' \<Longrightarrow>
@@ -101,7 +101,7 @@ proof (cases s')
         using RedSimpleCmdsCons_case
         by metis
 
-      then show ?thesis 
+      then show ?thesis
         using * by simp
     qed
   qed
@@ -110,13 +110,13 @@ proof (cases s')
     using RedSingleCmd \<open>s' = _\<close>
     by (auto intro: RedCmdListCons)
 
-  show ?thesis     
+  show ?thesis
     apply (rule exI, rule conjI)
      apply (rule converse_rtranclp_into_rtranclp)
     apply (subst \<open>s = _\<close>)
       apply (rule RedSimpleCmds)
     using RedList RedMultiEmptySimpleCmds \<open>s = _\<close> FailureConfig
-    by auto        
+    by auto
 next
   case Failure
   hence RedListFailure: "A, M, \<Lambda>, \<Gamma>, \<Omega> \<turnstile> \<langle>c#cs, s\<rangle> [\<rightarrow>] Failure"
@@ -125,16 +125,16 @@ next
   show ?thesis
   proof (cases s)
     case (Normal ns)
-    show ?thesis 
+    show ?thesis
       apply (subst Normal)
       apply (rule exI, rule conjI)
        apply (rule converse_rtranclp_into_rtranclp)
         apply (rule RedSimpleCmds)
       using RedListFailure Normal
-      by auto            
+      by auto
   next
     case Failure
-    then show ?thesis 
+    then show ?thesis
       by auto
   next
     case Magic
@@ -145,28 +145,28 @@ next
 next
   case Magic
   \<comment>\<open>cannot occur\<close>
-  then show ?thesis 
+  then show ?thesis
     using magic_stays_red_bigblock_multi assms
     by (metis RedMulti sndI state.distinct(5))
 qed
 
 lemma red_ast_block_red_bigblock_failure_preserve:
-  assumes "red_ast_bpl P ctxt c c'" and 
-          "snd c' = Failure" and 
-          "type_interp ctxt = A" and 
-          "var_context ctxt = \<Lambda>" and 
+  assumes "red_ast_bpl P ctxt c c'" and
+          "snd c' = Failure" and
+          "type_interp ctxt = A" and
+          "var_context ctxt = \<Lambda>" and
           "fun_interp ctxt = \<Gamma>"
           "rtype_interp ctxt = \<Omega>"
-        shows "\<exists>d'. red_bigblock_multi A ([] :: ast proc_context) \<Lambda> \<Gamma> \<Omega> P (fst (fst c), snd (fst c), snd c) d' 
+        shows "\<exists>d'. red_bigblock_multi A ([] :: ast proc_context) \<Lambda> \<Gamma> \<Omega> P (fst (fst c), snd (fst c), snd c) d'
                     \<and> (snd (snd d') = Failure)"
   using assms
   unfolding red_ast_bpl_def
 proof (induction rule: converse_rtranclp_induct)
   case base
-  then show ?case by auto    
+  then show ?case by auto
 next
   case (step y z)
-  from this obtain d' where    
+  from this obtain d' where
      Red2: "red_bigblock_multi A ([] :: ast proc_context) \<Lambda> \<Gamma> \<Omega> P (fst (fst z), snd (fst z), snd z) d'" and
      Red2StateFailure: "snd (snd d') = Failure"
     by blast
@@ -185,10 +185,10 @@ next
       by fastforce
   next
     case (RedBigBlockSmallNoSimpleCmdOneStep name str tr cont s b' cont' s')
-    then show ?thesis 
+    then show ?thesis
       using Red2 Red2StateFailure assms
       by (metis (no_types, lifting) converse_rtranclp_into_rtranclp fstI sndI step.prems(3))
-  qed           
+  qed
 qed
 
 lemma init_ast_convert_ast_to_program_point_eq:
@@ -205,27 +205,27 @@ lemma proc_body_satisfies_spec_valid_config:
   unfolding proc_body_satisfies_spec_def
   by blast
 
-text\<open>\<^const>\<open>Ast.proc_body_satisfies_spec\<close> is expressed via \<^const>\<open>red_bigblock\<close>, while \<^const>\<open>red_ast_bpl\<close> 
+text\<open>\<^const>\<open>Ast.proc_body_satisfies_spec\<close> is expressed via \<^const>\<open>red_bigblock\<close>, while \<^const>\<open>red_ast_bpl\<close>
      is expressed via \<^const>\<open>red_bigblock_small\<close>. The following lemma bridges the gap.\<close>
 
 lemma red_ast_bpl_proc_body_sat_spec:
   assumes RedBpl: "red_ast_bpl proc_body_ast ctxt (convert_ast_to_program_point proc_body_ast, Normal ns) c'" and
           PreconditionsSat: "expr_all_sat (type_interp ctxt) (var_context ctxt) (fun_interp ctxt) (rtype_interp ctxt) ns pres" and
-          ProcBodySatSpec: "(Ast.proc_body_satisfies_spec :: (('a vbpl_absval, ast) proc_body_satisfies_spec_ty)) (type_interp ctxt) [] (var_context ctxt) (fun_interp ctxt) (rtype_interp ctxt) 
+          ProcBodySatSpec: "(Ast.proc_body_satisfies_spec :: (('a vbpl_absval, ast) proc_body_satisfies_spec_ty)) (type_interp ctxt) [] (var_context ctxt) (fun_interp ctxt) (rtype_interp ctxt)
                                        pres posts proc_body_ast ns"
         shows "snd c' \<noteq> Failure"
 proof (rule ccontr)
   assume "\<not> snd c' \<noteq> Failure"
   hence "snd c' = Failure"
     by simp
-    
-  obtain d' where 
+
+  obtain d' where
     RedBigBlockMulti: "(red_bigblock_multi (type_interp ctxt) ([] :: ast proc_context) (var_context ctxt) (fun_interp ctxt) (rtype_interp ctxt) proc_body_ast)\<^sup>*\<^sup>*
        (init_ast proc_body_ast ns) d'" and
-    "snd (snd d') = Failure"  
+    "snd (snd d') = Failure"
         using red_ast_block_red_bigblock_failure_preserve[OF RedBpl \<open>snd c' = _\<close>] init_ast_convert_ast_to_program_point_eq
         by (metis fstI r_into_rtranclp sndI)
-      
+
   let ?d'_bigblock = "fst d'"
   let ?d'_cont = "fst (snd d')"
   let ?d'_state = "snd (snd d')"
@@ -238,7 +238,7 @@ proof (rule ccontr)
     by auto
   thus False
     using \<open>snd (snd d') = Failure\<close> valid_configuration_not_failure
-    by blast 
+    by blast
 qed
 
 definition post_framing_rel_aux
@@ -250,9 +250,9 @@ definition post_framing_rel_aux
 
 definition post_framing_rel
   where "post_framing_rel ctxt_vpr StateCons \<Lambda> proc_body_bpl ctxt mdecl R0 \<gamma>Pre \<equiv>
-           (\<forall>\<omega>0 \<omega>1 ns. R0 \<omega>0 ns \<longrightarrow> get_store_total \<omega>0 = get_store_total \<omega>1 \<longrightarrow> 
+           (\<forall>\<omega>0 \<omega>1 ns. R0 \<omega>0 ns \<longrightarrow> get_store_total \<omega>0 = get_store_total \<omega>1 \<longrightarrow>
                                \<comment>\<open>One could omit emptiness and instead use a separate monotonicity theorem
-                                  for inhale. We do this in a separate step.\<close> 
+                                  for inhale. We do this in a separate step.\<close>
                                is_empty_total_full \<omega>1 \<longrightarrow>
                                StateCons \<omega>1 \<longrightarrow>  \<comment> \<open>ForMe: Hope it makes sense.\<close>
                                total_heap_well_typed (program_total ctxt_vpr) (absval_interp_total ctxt_vpr) (get_hh_total_full \<omega>1) \<longrightarrow>
@@ -260,28 +260,28 @@ definition post_framing_rel
                    )"
 
 definition method_rel
-  where "method_rel R0 R1 ctxt_vpr StateCons \<Lambda> proc_body_bpl ctxt mdecl \<gamma>0 \<equiv> 
+  where "method_rel R0 R1 ctxt_vpr StateCons \<Lambda> proc_body_bpl ctxt mdecl \<gamma>0 \<equiv>
           (\<exists> \<gamma>Pre. stmt_rel R0 R1 ctxt_vpr StateCons \<Lambda> proc_body_bpl ctxt (Inhale (method_decl.pre mdecl)) \<gamma>0 \<gamma>Pre \<and>
                    post_framing_rel ctxt_vpr StateCons \<Lambda> proc_body_bpl ctxt mdecl R1 \<gamma>Pre \<and>
-                   (  \<comment>\<open>The correctness of the spec must be taken into account in this left-hand side here and 
-                         not in a previous conjunct, since the previous conjunct is required to justify the 
+                   (  \<comment>\<open>The correctness of the spec must be taken into account in this left-hand side here and
+                         not in a previous conjunct, since the previous conjunct is required to justify the
                          correctness of the spec.
                          We need this left-hand side, because the Boogie encoding may rely on the correctness
-                         of the specs.\<close> 
+                         of the specs.\<close>
                       method_decl.body mdecl \<noteq> None \<longrightarrow> \<comment>\<open>correctness of body is relevant only if the method has a body\<close>
-                      vpr_all_method_spec_correct_total ctxt_vpr StateCons (program_total ctxt_vpr) \<longrightarrow> 
+                      vpr_all_method_spec_correct_total ctxt_vpr StateCons (program_total ctxt_vpr) \<longrightarrow>
                       (\<exists>\<gamma>Body \<gamma>Post R1'. \<comment>\<open>output Boogie program point and output relation are irrelevant\<close>
-                         stmt_rel R1 R1 ctxt_vpr StateCons \<Lambda> proc_body_bpl ctxt (the (method_decl.body mdecl)) \<gamma>Pre \<gamma>Body \<and>    
+                         stmt_rel R1 R1 ctxt_vpr StateCons \<Lambda> proc_body_bpl ctxt (the (method_decl.body mdecl)) \<gamma>Pre \<gamma>Body \<and>
                           \<comment>\<open>because framedness of the postcondition was checked above, we may use it here.
-                             TODO: could make sense to abstract \<^const>\<open>framing_exh\<close> away via a parameter\<close>                   
-                         stmt_rel (\<lambda> \<omega> ns. R1 \<omega> ns \<and> framing_exh ctxt_vpr StateCons (method_decl.post mdecl) \<omega> \<omega>) 
+                             TODO: could make sense to abstract \<^const>\<open>framing_exh\<close> away via a parameter\<close>
+                         stmt_rel (\<lambda> \<omega> ns. R1 \<omega> ns \<and> framing_exh ctxt_vpr StateCons (method_decl.post mdecl) \<omega> \<omega>)
                                   R1' ctxt_vpr StateCons \<Lambda> proc_body_bpl ctxt (Exhale (method_decl.post mdecl)) \<gamma>Body \<gamma>Post
                       )
                    )
           )"
 
 lemma post_framing_rel_aux:
-  assumes WfTyRep: "wf_ty_repr_bpl TyRep" 
+  assumes WfTyRep: "wf_ty_repr_bpl TyRep"
       and WfConsistency: "wf_total_consistency ctxt_vpr StateCons StateCons_t"
       and TypeInterp: "type_interp ctxt = vbpl_absval_ty TyRep"
       and "domain_type TyRep = absval_interp_total ctxt_vpr"
@@ -296,17 +296,17 @@ lemma post_framing_rel_aux:
                               (range (const_repr Tr)) \<union>
                               dom AuxPred) = {}" (is "?A \<inter> ?B = {}")
       and "hvar' \<noteq> mvar'"
-      and PropagateBpl: "red_ast_bpl_rel (state_rel_well_def_same ctxt Pr StateCons (TyRep :: 'a ty_repr_bpl) Tr AuxPred) 
-                                         (state_rel_well_def_same ctxt Pr StateCons (TyRep :: 'a ty_repr_bpl) Tr AuxPred) proc_body_bpl ctxt 
-                                         \<gamma>Pre 
+      and PropagateBpl: "red_ast_bpl_rel (state_rel_well_def_same ctxt Pr StateCons (TyRep :: 'a ty_repr_bpl) Tr AuxPred)
+                                         (state_rel_well_def_same ctxt Pr StateCons (TyRep :: 'a ty_repr_bpl) Tr AuxPred) proc_body_bpl ctxt
+                                         \<gamma>Pre
                                          (BigBlock name (Havoc hvar' # Assign mvar' (Var zero_mask_var) # cs) str tr, cont)"
-      and PostInhRel: 
+      and PostInhRel:
              "stmt_rel (state_rel_well_def_same ctxt Pr StateCons TyRep (Tr\<lparr>heap_var := hvar', mask_var := mvar', heap_var_def := hvar', mask_var_def := mvar'\<rparr>) AuxPred)
                        R' ctxt_vpr StateCons \<Lambda> proc_body_bpl ctxt
                        (Inhale (method_decl.post mdecl))
                        (BigBlock name cs str tr, cont)
-                       \<gamma>'" 
-    shows "post_framing_rel ctxt_vpr StateCons \<Lambda> proc_body_bpl ctxt mdecl 
+                       \<gamma>'"
+    shows "post_framing_rel ctxt_vpr StateCons \<Lambda> proc_body_bpl ctxt mdecl
                             (state_rel_well_def_same ctxt Pr StateCons (TyRep :: 'a ty_repr_bpl) Tr AuxPred)
                           \<gamma>Pre"
   unfolding post_framing_rel_def
@@ -319,15 +319,15 @@ proof (rule allI | rule impI)+
          IsEmpty: "is_empty_total_full \<omega>1" and
          IntCons: "StateCons \<omega>1"
 
-  with PropagateBpl obtain ns1 where 
-    RedBpl1: "red_ast_bpl proc_body_bpl ctxt 
+  with PropagateBpl obtain ns1 where
+    RedBpl1: "red_ast_bpl proc_body_bpl ctxt
                               (\<gamma>Pre, Normal ns)
                               ((BigBlock name (Havoc hvar' # Assign mvar' (Var zero_mask_var) # cs) str tr, cont), Normal ns1)" and
     R1: "?R Tr \<omega>0 ns1"
     unfolding red_ast_bpl_rel_def
     by blast
 
-  have *: "\<And>\<omega>0 \<omega> ns hvar' hvar. state_rel Pr StateCons TyRep ((disable_consistent_state_rel_opt Tr)\<lparr>heap_var := hvar, heap_var_def := hvar'\<rparr>) AuxPred ctxt \<omega>0 \<omega> ns \<Longrightarrow> 
+  have *: "\<And>\<omega>0 \<omega> ns hvar' hvar. state_rel Pr StateCons TyRep ((disable_consistent_state_rel_opt Tr)\<lparr>heap_var := hvar, heap_var_def := hvar'\<rparr>) AuxPred ctxt \<omega>0 \<omega> ns \<Longrightarrow>
                     red_expr_bpl ctxt (Var zero_mask_var) ns (AbsV (AMask zero_mask_bpl))"
     apply (rule RedVar)
     using boogie_const_rel_lookup[OF state_rel_boogie_const_rel, where ?const = CZeroMask]
@@ -350,14 +350,14 @@ proof (rule allI | rule impI)+
         ((BigBlock name (cmd.Havoc hvar' # Assign mvar' (expr.Var zero_mask_var) # cs) str tr, cont),
          Normal ns1)
         ((BigBlock name cs str tr, cont), Normal ns2)" and
-    R2: "?R (Tr\<lparr>heap_var := hvar', mask_var := mvar', heap_var_def := hvar', mask_var_def := mvar'\<rparr>) \<omega>1 ns2"             
-    using is_empty_total_wf_mask[OF IsEmpty] 
+    R2: "?R (Tr\<lparr>heap_var := hvar', mask_var := mvar', heap_var_def := hvar', mask_var_def := mvar'\<rparr>) \<omega>1 ns2"
+    using is_empty_total_wf_mask[OF IsEmpty]
     by force
-    
+
   with RedBpl1 have RedBpl2: "red_ast_bpl proc_body_bpl ctxt (\<gamma>Pre, Normal ns) ((BigBlock name cs str tr, cont), Normal ns2)"
     using red_ast_bpl_transitive
     by fast
-   
+
   show "post_framing_rel_aux ctxt_vpr StateCons \<Lambda> proc_body_bpl ctxt mdecl (?R Tr) \<gamma>Pre \<omega>1 ns"
     unfolding post_framing_rel_aux_def
     apply ((rule exI)+, intro conjI)
@@ -375,10 +375,10 @@ lemma post_framing_rel_framing_trivial:
 
 definition vpr_method_correct_total_partial :: "'a total_context \<Rightarrow> ('a full_total_state \<Rightarrow> bool) \<Rightarrow> method_decl \<Rightarrow> bool" where
   "vpr_method_correct_total_partial ctxt StateCons mdecl \<equiv>
-         vpr_method_correct_total_aux ctxt StateCons mdecl 
+         vpr_method_correct_total_aux ctxt StateCons mdecl
           (\<lambda>ctxt R mdecl \<omega>pre \<omega>.
                 vpr_postcondition_framed ctxt R (method_decl.post mdecl) (get_total_full \<omega>pre) (get_store_total \<omega>) \<and>
-                (method_decl.body mdecl \<noteq> None \<longrightarrow> 
+                (method_decl.body mdecl \<noteq> None \<longrightarrow>
                  vpr_all_method_spec_correct_total ctxt StateCons (program_total ctxt) \<longrightarrow>
                  vpr_method_body_correct ctxt R mdecl \<omega>pre)
           )
@@ -396,7 +396,7 @@ proof -
     assume "methods (program_total ctxt) m = Some mdecl"
     hence "vpr_method_correct_total_partial ctxt StateCons mdecl"
       using assms
-      by blast    
+      by blast
     thus "vpr_method_spec_correct_total ctxt StateCons mdecl"
       unfolding vpr_method_correct_total_partial_def vpr_method_spec_correct_total_def vpr_method_correct_total_aux_def
       by blast
@@ -416,10 +416,10 @@ qed
 subsection \<open>Main helper lemma for final theorem\<close>
 
 lemma end_to_end_vpr_method_correct_partial:
-  assumes 
+  assumes
           \<comment>\<open>The Boogie procedure is correct. Note that we need to explicitly provide the types such that
              we can then instantiate the Boogie type interpretation with \<^term>\<open>vbpl_absval_ty TyRep\<close>.\<close>
-          Boogie_correct: "proc_is_correct (vbpl_absval_ty (TyRep :: 'a ty_repr_bpl)) fun_decls constants unique_consts global_vars axioms (proc_bpl :: ast procedure) 
+          Boogie_correct: "proc_is_correct (vbpl_absval_ty (TyRep :: 'a ty_repr_bpl)) fun_decls constants unique_consts global_vars axioms (proc_bpl :: ast procedure)
                   (Ast.proc_body_satisfies_spec :: (('a vbpl_absval, ast) proc_body_satisfies_spec_ty))"
       and ConsistencyDownwardMono: "mono_prop_downward_ord StateCons"
       and WfTyRep: "wf_ty_repr_bpl TyRep"
@@ -432,13 +432,13 @@ lemma end_to_end_vpr_method_correct_partial:
       and VprNoPermSupportedSpec: "no_perm_assertion (method_decl.pre mdecl) \<and> supported_assertion (method_decl.pre mdecl) \<and>
                                    no_perm_assertion (method_decl.post mdecl) \<and> supported_assertion (method_decl.post mdecl)"
       and OnlyArgsInPre: "\<And> x. x \<in> free_var_assertion (method_decl.pre mdecl) \<Longrightarrow> x < length (method_decl.args mdecl)"
-      and ArgsUnmodified: "method_decl.body mdecl \<noteq> None \<Longrightarrow> 
+      and ArgsUnmodified: "method_decl.body mdecl \<noteq> None \<Longrightarrow>
                                   (\<And>x. x < length (method_decl.args mdecl) \<Longrightarrow> x \<notin> modif body_vpr)"
-      and "\<Lambda> = nth_option (method_decl.args mdecl @ rets mdecl)"      
+      and "\<Lambda> = nth_option (method_decl.args mdecl @ rets mdecl)"
 
 \<comment>\<open>Boogie properties\<close>
       and FunInterp: "fun_interp_wf (vbpl_absval_ty TyRep) fun_decls (fun_interp ctxt)"
-      and TypeInterpEq: "type_interp ctxt = vbpl_absval_ty TyRep"  
+      and TypeInterpEq: "type_interp ctxt = vbpl_absval_ty TyRep"
       and "rtype_interp ctxt = []"
       and VarCtxtEq: "var_context ctxt = (constants @ global_vars, proc_args proc_bpl @ locals_bpl @ proc_rets proc_bpl)"
           \<comment>\<open>The Viper encoding does not use Boogie procedure preconditions\<close>
@@ -447,22 +447,22 @@ lemma end_to_end_vpr_method_correct_partial:
       and ProcBodySome: "proc_body proc_bpl = Some (locals_bpl, proc_body_bpl)"
 
 \<comment>\<open>method rel\<close>
-      and VprMethodRel: "method_rel 
+      and VprMethodRel: "method_rel
                (state_rel_empty (state_rel_well_def_same ctxt (program_total ctxt_vpr) StateCons (TyRep :: 'a ty_repr_bpl) Tr AuxPred))
                (state_rel_well_def_same ctxt (program_total ctxt_vpr) StateCons (TyRep :: 'a ty_repr_bpl) Tr AuxPred)
-               ctxt_vpr StateCons \<Lambda> proc_body_bpl ctxt mdecl               
-               (convert_ast_to_program_point proc_body_bpl)" 
+               ctxt_vpr StateCons \<Lambda> proc_body_bpl ctxt mdecl
+               (convert_ast_to_program_point proc_body_bpl)"
           (is "method_rel ?R0 ?R1 ctxt_vpr StateCons \<Lambda> proc_body_bpl ctxt mdecl ?\<gamma>0")
       and ConsistencyEnabled: "consistent_state_rel_opt (state_rel_opt Tr)"
 
 \<comment>\<open>construct initial state\<close>
-      and InitialStateRel: "\<And> \<omega>.  
+      and InitialStateRel: "\<And> \<omega>.
                        vpr_store_well_typed (absval_interp_total ctxt_vpr) (nth_option (method_decl.args mdecl @ rets mdecl)) (get_store_total \<omega>) \<Longrightarrow>
                        total_heap_well_typed (program_total ctxt_vpr) (absval_interp_total ctxt_vpr) (get_hh_total_full \<omega>) \<Longrightarrow>
                        is_empty_total_full \<omega> \<Longrightarrow>
                        StateCons \<omega> \<Longrightarrow>
                        \<exists>ns ls gs.
-                           ns = \<lparr>old_global_state = gs, global_state = gs, local_state = ls, binder_state = Map.empty\<rparr> \<and>  
+                           ns = \<lparr>old_global_state = gs, global_state = gs, local_state = ls, binder_state = Map.empty\<rparr> \<and>
                            \<comment>\<open>well-typedness of Boogie state follows from state relation\<close>
                            (state_rel_empty (state_rel_well_def_same ctxt (program_total ctxt_vpr) StateCons (TyRep :: 'a ty_repr_bpl) Tr AuxPred)) \<omega> ns \<and>
                            unique_constants_distinct gs unique_consts \<and>
@@ -474,7 +474,7 @@ proof (rule allI | rule impI)+
 
   let ?R1Post = "\<lambda>\<omega> ns. ?R1 \<omega> ns \<and> framing_exh ctxt_vpr StateCons (method_decl.post mdecl) \<omega> \<omega>"
 
-  from VprMethodRel obtain \<gamma>Pre \<gamma>Body \<gamma>Post Rend where 
+  from VprMethodRel obtain \<gamma>Pre \<gamma>Body \<gamma>Post Rend where
     PreInhRel: "stmt_rel ?R0 ?R1 ctxt_vpr StateCons \<Lambda> proc_body_bpl ctxt (Inhale (method_decl.pre mdecl)) ?\<gamma>0 \<gamma>Pre" and
     PostFramingRel: "post_framing_rel ctxt_vpr StateCons \<Lambda> proc_body_bpl ctxt mdecl ?R1 \<gamma>Pre" and
     BodyRel: "method_decl.body mdecl \<noteq> None \<Longrightarrow>
@@ -485,7 +485,7 @@ proof (rule allI | rule impI)+
               stmt_rel ?R1Post Rend ctxt_vpr StateCons \<Lambda> proc_body_bpl ctxt (Exhale (method_decl.post mdecl)) \<gamma>Body \<gamma>Post"
     unfolding method_rel_def
     using VprMethodBody
-    by fastforce   
+    by fastforce
 
   text \<open>start actual proof\<close>
 
@@ -497,14 +497,14 @@ proof (rule allI | rule impI)+
          "is_empty_total_full \<omega>" and
          "StateCons \<omega>" and
          RedInhPre: "red_inhale ctxt_vpr StateCons (method_decl.pre mdecl) \<omega> rpre"
-  
+
   let ?abs = "vbpl_absval_ty TyRep"
 
   note Boogie_correct_inst=Boogie_correct
 
-  obtain ns ls gs where 
+  obtain ns ls gs where
     "ns = \<lparr>old_global_state = gs, global_state = gs, local_state = ls, binder_state = Map.empty\<rparr>" and
-  StateRelInitialInst: 
+  StateRelInitialInst:
     "state_rel_empty (state_rel_well_def_same ctxt (program_total ctxt_vpr) StateCons (TyRep :: 'a ty_repr_bpl) Tr AuxPred) \<omega> ns" and
   UniqueConstants:
     "unique_constants_distinct gs unique_consts" and
@@ -515,16 +515,16 @@ proof (rule allI | rule impI)+
 
   from StateRelInitialInst have StateRel: "state_rel (program_total ctxt_vpr) StateCons TyRep Tr AuxPred ctxt \<omega> \<omega> ns"
     by (simp add: state_rel_empty_def)
-    
+
   have
     GlobalsWf: "state_typ_wf (vbpl_absval_ty TyRep) [] gs (constants @ global_vars)" and
     LocalsWf: "state_typ_wf (vbpl_absval_ty TyRep) [] ls ((proc_args proc_bpl)@ (locals_bpl @ proc_rets proc_bpl))"
     using state_rel_state_well_typed[OF StateRel] \<open>ns = _\<close> VarCtxtEq TypeInterpEq
-    unfolding state_rel_empty_def state_well_typed_def 
-    by auto          
-  
+    unfolding state_rel_empty_def state_well_typed_def
+    by auto
+
   have ProcBodyBplCorrect:
-      "(Ast.proc_body_satisfies_spec :: (('a vbpl_absval, ast) proc_body_satisfies_spec_ty)) ?abs [] (constants@global_vars, (proc_args proc_bpl)@(locals_bpl@(proc_rets proc_bpl))) (fun_interp ctxt) [] 
+      "(Ast.proc_body_satisfies_spec :: (('a vbpl_absval, ast) proc_body_satisfies_spec_ty)) ?abs [] (constants@global_vars, (proc_args proc_bpl)@(locals_bpl@(proc_rets proc_bpl))) (fun_interp ctxt) []
                                        (proc_all_pres proc_bpl) (proc_checked_posts proc_bpl) proc_body_bpl
                                        \<lparr>old_global_state = gs, global_state = gs, local_state = ls, binder_state = Map.empty\<rparr>"
   proof (rule proc_is_correct_elim[OF Boogie_correct_inst ProcBodySome])
@@ -540,7 +540,7 @@ proof (rule allI | rule impI)+
         then show ?thesis by simp
       next
         case (AbsV x2)
-        then show ?thesis 
+        then show ?thesis
           using vbpl_absval_ty_closed[OF WfTyRep]
           by fastforce
       qed
@@ -554,7 +554,7 @@ proof (rule allI | rule impI)+
   next
     show "state_typ_wf (vbpl_absval_ty TyRep) [] gs (constants @ global_vars)"
       by (rule GlobalsWf)
-  next 
+  next
     show "state_typ_wf (vbpl_absval_ty TyRep) [] ls (proc_args proc_bpl @ locals_bpl @ proc_rets proc_bpl)"
       by (rule LocalsWf)
   next
@@ -568,7 +568,7 @@ proof (rule allI | rule impI)+
   show "rpre \<noteq> RFailure \<and>
        (\<forall>\<omega>pre.
            rpre = RNormal \<omega>pre \<longrightarrow>
-           vpr_postcondition_framed ctxt_vpr StateCons (method_decl.post mdecl) (get_total_full \<omega>pre) (get_store_total \<omega>) \<and> 
+           vpr_postcondition_framed ctxt_vpr StateCons (method_decl.post mdecl) (get_total_full \<omega>pre) (get_store_total \<omega>) \<and>
            (method_decl.body mdecl \<noteq> None \<longrightarrow> vpr_all_method_spec_correct_total ctxt_vpr StateCons (program_total ctxt_vpr) \<longrightarrow>
             vpr_method_body_correct ctxt_vpr StateCons mdecl \<omega>pre)
         )"
@@ -581,10 +581,10 @@ proof (rule allI | rule impI)+
       hence "rpre = RFailure" by simp
       with stmt_rel_failure_elim[OF PreInhRel StateRelInitialInst] RedInhPre
        obtain c' where
-        FailureConfig: "snd c' = Failure" and 
+        FailureConfig: "snd c' = Failure" and
         RedBpl: "red_ast_bpl proc_body_bpl ctxt (convert_ast_to_program_point proc_body_bpl, Normal ns) c'"
         using RedInhale
-        by blast  
+        by blast
 
       have "snd c' \<noteq> Failure"
         using red_ast_bpl_proc_body_sat_spec[OF RedBpl, where ?pres="(Ast.proc_all_pres proc_bpl)"]
@@ -594,7 +594,7 @@ proof (rule allI | rule impI)+
 
       thus False
         using \<open>snd c' = Failure\<close>
-        by simp 
+        by simp
     qed
   next
     show ?Goal2
@@ -619,7 +619,7 @@ proof (rule allI | rule impI)+
         fix \<phi> trace res
         let ?\<omega>Post = "\<lparr>get_store_total = get_store_total \<omega>, get_trace_total = trace, get_total_full = \<phi>\<rparr>"
         let ?\<omega>PostEmpty = "empty_full_total_state (get_store_total \<omega>) trace (get_hh_total \<phi>)"
-        assume 
+        assume
               "total_heap_well_typed (program_total ctxt_vpr) (absval_interp_total ctxt_vpr) (get_hh_total \<phi>)"
           and TraceOldState: "trace old_label = Some (get_total_full \<omega>pre)"
           and \<omega>preCons: "StateCons \<lparr> get_store_total = get_store_total \<omega>, get_trace_total = trace, get_total_full = \<phi> \<rparr>"
@@ -628,7 +628,7 @@ proof (rule allI | rule impI)+
         hence HeapWellTy: "total_heap_well_typed (program_total ctxt_vpr) (absval_interp_total ctxt_vpr) (get_hh_total_full ?\<omega>PostEmpty)"
           by (simp add: empty_full_total_state_def)
 
-        from PostFramingRel obtain ns' \<gamma>Framing0 \<gamma>Framing1 RPostFrameStart RPostFrameEnd where 
+        from PostFramingRel obtain ns' \<gamma>Framing0 \<gamma>Framing1 RPostFrameStart RPostFrameEnd where
           RedPreToFramingBpl: "red_ast_bpl proc_body_bpl ctxt (\<gamma>Pre, Normal nspre) (\<gamma>Framing0, Normal ns')" and
           "RPostFrameStart ?\<omega>PostEmpty ns'" and
           PostFramingInhRel: "stmt_rel RPostFrameStart RPostFrameEnd ctxt_vpr StateCons \<Lambda> proc_body_bpl ctxt (Inhale (method_decl.post mdecl)) \<gamma>Framing0 \<gamma>Framing1"
@@ -646,17 +646,17 @@ proof (rule allI | rule impI)+
             apply (rule is_empty_total_full_less_eq)
             by (simp_all add: empty_full_total_state_def is_empty_total_def)
 
-          with inhale_no_perm_downwards_mono ConsistencyDownwardMono RedInhPost 
+          with inhale_no_perm_downwards_mono ConsistencyDownwardMono RedInhPost
           have "red_inhale ctxt_vpr StateCons (method_decl.post mdecl) ?\<omega>PostEmpty RFailure"
             using is_empty_empty_full_total_state \<open>res = _\<close>  VprNoPermSupportedSpec supported_assertion_no_unfolding
             by blast
-            
+
           with stmt_rel_failure_elim[OF PostFramingInhRel \<open>RPostFrameStart _ _\<close>]
-          obtain c' where "red_ast_bpl proc_body_bpl ctxt (\<gamma>Framing0, Normal ns') c'" and 
+          obtain c' where "red_ast_bpl proc_body_bpl ctxt (\<gamma>Framing0, Normal ns') c'" and
                           "snd c' = Failure"
             using RedInhale \<open>\<Lambda> = _\<close>
             by blast
-            
+
           with RedPreBpl RedPreToFramingBpl
           have RedBpl: "red_ast_bpl proc_body_bpl ctxt (convert_ast_to_program_point proc_body_bpl, Normal ns) c'"
             using red_ast_bpl_transitive
@@ -667,7 +667,7 @@ proof (rule allI | rule impI)+
               ProcPresEmpty ProcBodyBplCorrect
             unfolding expr_all_sat_def
             by (simp add: \<open>var_context _ = _\<close> \<open>type_interp _ = _\<close> \<open>rtype_interp _ =_\<close> \<open>ns = _\<close>)
-          thus False 
+          thus False
             by (simp add: \<open>snd c' = Failure\<close>)
         qed
       qed
@@ -680,8 +680,8 @@ proof (rule allI | rule impI)+
         let ?mbody = "(the (method_decl.body mdecl))"
         fix rpost
         assume "method_decl.body mdecl \<noteq> None"
-           and SpecsCorrect: "vpr_all_method_spec_correct_total ctxt_vpr StateCons (program_total ctxt_vpr)"   
-           and RedBodyVpr: "red_stmt_total ctxt_vpr StateCons ?\<Lambda> 
+           and SpecsCorrect: "vpr_all_method_spec_correct_total ctxt_vpr StateCons (program_total ctxt_vpr)"
+           and RedBodyVpr: "red_stmt_total ctxt_vpr StateCons ?\<Lambda>
                                (Seq ?mbody (Exhale (method_decl.post mdecl)))
                                ?\<omega>pre' rpost"
 
@@ -702,37 +702,37 @@ proof (rule allI | rule impI)+
             using Rpre
             by blast
         qed
- 
+
         show "rpost \<noteq> RFailure"
         proof (rule ccontr)
           assume "\<not> rpost \<noteq> RFailure"
           hence "rpost = RFailure" by simp
-          with RedBodyVpr 
+          with RedBodyVpr
           have RedCasesVpr: "red_stmt_total ctxt_vpr StateCons ?\<Lambda> ?mbody ?\<omega>pre' RFailure \<or>
                (\<exists>\<omega>body. red_stmt_total ctxt_vpr StateCons ?\<Lambda> ?mbody ?\<omega>pre' (RNormal \<omega>body) \<and>
                         red_stmt_total ctxt_vpr StateCons ?\<Lambda> (Exhale (method_decl.post mdecl)) \<omega>body RFailure)"
             (is "?Case1 \<or> ?Case2")
             by (auto elim: red_stmt_total_inversion_thms)
-          
+
           show False
           proof (rule disjE[OF RedCasesVpr])
             assume ?Case1
-   
-            with stmt_rel_failure_elim[OF BodyRel Rpre_old_upd] RedBodyVpr obtain c' 
+
+            with stmt_rel_failure_elim[OF BodyRel Rpre_old_upd] RedBodyVpr obtain c'
               where "snd c' = Failure" and "red_ast_bpl proc_body_bpl ctxt (\<gamma>Pre, Normal nspre) c'"
               using \<open>\<Lambda> = _\<close> VprMethodBodySome SpecsCorrect
               by fastforce
-  
+
             hence RedBpl: "red_ast_bpl proc_body_bpl ctxt (convert_ast_to_program_point proc_body_bpl, Normal ns) c'"
               using RedPreBpl red_ast_bpl_transitive
               by blast
-  
+
             have "snd c' \<noteq> Failure"
               using red_ast_bpl_proc_body_sat_spec[OF RedBpl, where ?pres="(Ast.proc_all_pres proc_bpl)"]
                 ProcPresEmpty ProcBodyBplCorrect
               unfolding expr_all_sat_def
               by (simp add: \<open>var_context _ = _\<close> \<open>type_interp _ = _\<close> \<open>rtype_interp _ =_\<close> \<open>ns = _\<close>)
-            thus False 
+            thus False
               by (simp add: \<open>snd c' = Failure\<close>)
           next
             assume ?Case2
@@ -742,7 +742,7 @@ proof (rule allI | rule impI)+
               by (auto elim: red_stmt_total_inversion_thms)
 
             from stmt_rel_normal_elim[OF BodyRel Rpre_old_upd] RedBodyVpr obtain nsbody
-              where 
+              where
                RedBodyBpl: "red_ast_bpl proc_body_bpl ctxt (\<gamma>Pre, Normal nspre) (\<gamma>Body, Normal nsbody)" and
                Rbody: "state_rel_well_def_same ctxt (program_total ctxt_vpr) StateCons TyRep Tr AuxPred \<omega>body nsbody"
               using \<open>\<Lambda> = _\<close> VprMethodBodySome SpecsCorrect
@@ -751,7 +751,7 @@ proof (rule allI | rule impI)+
             have FramingExhPost: "framing_exh ctxt_vpr StateCons (method_decl.post mdecl) \<omega>body \<omega>body"
             proof (rule framing_exhI_state_rel[OF Rbody ConsistencyEnabled])
 
-              from SpecsCorrect and ProgMethod 
+              from SpecsCorrect and ProgMethod
               have SpecCorrectMdecl: "vpr_method_spec_correct_total ctxt_vpr StateCons mdecl"
                 unfolding vpr_all_method_spec_correct_total_def
                 by blast
@@ -772,18 +772,18 @@ proof (rule allI | rule impI)+
                   using red_stmt_preserves_unmodified_variables VprMethodBodySome RedBodyVpr \<open>get_store_total \<omega>pre = get_store_total \<omega>\<close>
                   by fastforce
                 thus "?B x"
-                  by simp           
-              qed                
+                  by simp
+              qed
 
               with OnlyArgsInPre VprNoPermSupportedSpec RedInhPre \<open>rpre = RNormal \<omega>pre\<close>
-              have RedInhStoreBody: "red_inhale ctxt_vpr StateCons (method_decl.pre mdecl) 
+              have RedInhStoreBody: "red_inhale ctxt_vpr StateCons (method_decl.pre mdecl)
                         ?\<omega>_store_body (RNormal (\<omega>pre \<lparr> get_store_total := get_store_total \<omega>body \<rparr>))"
                 using red_inhale_store_same_on_free_var[OF RedInhPre _ StoresAgreeOnArgs] WfConsistency
                 by simp
-                
-              hence 
+
+              hence
                PostFramedStoreBody: "vpr_postcondition_framed ctxt_vpr StateCons (method_decl.post mdecl) (get_total_full (\<omega>pre\<lparr>get_store_total := get_store_total \<omega>body\<rparr>))
-                                                                                     (get_store_total ?\<omega>_store_body)"            
+                                                                                     (get_store_total ?\<omega>_store_body)"
               proof (rule vpr_method_correct_total_aux_normalD[OF SpecCorrectMdecl[simplified vpr_method_spec_correct_total_def]])
                 show "vpr_store_well_typed (absval_interp_total ctxt_vpr) (nth_option (method_decl.args mdecl @ rets mdecl)) (get_store_total ?\<omega>_store_body)"
                   apply simp
@@ -791,7 +791,7 @@ proof (rule allI | rule impI)+
                   by (metis update_trace_total_store_same)
               next
                 show "total_heap_well_typed (program_total ctxt_vpr) (absval_interp_total ctxt_vpr) (get_hh_total_full (\<omega>\<lparr>get_store_total := get_store_total \<omega>body\<rparr>))"
-                  using HeapWellTy 
+                  using HeapWellTy
                   by simp
               next
                 show "is_empty_total_full (\<omega>\<lparr>get_store_total := get_store_total \<omega>body\<rparr>)"
@@ -808,8 +808,8 @@ proof (rule allI | rule impI)+
 
               show "assertion_framing_state ctxt_vpr StateCons (method_decl.post mdecl) (upd_nm_total_full \<omega>body 0)"
               proof (rule vpr_postcondition_framed_assertion_framing_state[OF PostFramedStoreBody])
-                show "upd_nm_total_full \<omega>body 0 = 
-                     \<lparr>get_store_total = get_store_total (\<omega>\<lparr>get_store_total := get_store_total \<omega>body\<rparr>), get_trace_total = get_trace_total \<omega>body, 
+                show "upd_nm_total_full \<omega>body 0 =
+                     \<lparr>get_store_total = get_store_total (\<omega>\<lparr>get_store_total := get_store_total \<omega>body\<rparr>), get_trace_total = get_trace_total \<omega>body,
                                                            get_total_full = ?\<phi>\<rparr>"
                   by auto
               next
@@ -847,9 +847,9 @@ proof (rule allI | rule impI)+
             qed (auto simp: DomainType)
 
             with stmt_rel_failure_elim[OF PostExhRel]
-            obtain c' where "snd c' = Failure" and 
+            obtain c' where "snd c' = Failure" and
                             "red_ast_bpl proc_body_bpl ctxt (\<gamma>Body, Normal nsbody) c'"
-              using Rbody VprMethodBodySome FramingExhPost RedExhPost RedExhaleFailure SpecsCorrect 
+              using Rbody VprMethodBodySome FramingExhPost RedExhPost RedExhaleFailure SpecsCorrect
               by blast
 
             hence RedBpl: "red_ast_bpl proc_body_bpl ctxt (convert_ast_to_program_point proc_body_bpl, Normal ns) c'"
@@ -861,7 +861,7 @@ proof (rule allI | rule impI)+
               ProcPresEmpty ProcBodyBplCorrect
             unfolding expr_all_sat_def
             by (simp add: \<open>var_context _ = _\<close> \<open>type_interp _ = _\<close> \<open>rtype_interp _ =_\<close> \<open>ns = _\<close>)
-            thus False 
+            thus False
               by (simp add: \<open>snd c' = Failure\<close>)
           qed
         qed
@@ -873,13 +873,13 @@ qed
   subsection \<open>General setup for constructing well-typed states\<close>
 
 fun named_state_var_context :: "'a absval_ty_fun \<Rightarrow> vdecls \<Rightarrow> 'a named_state"
-  where "named_state_var_context A vs x = 
+  where "named_state_var_context A vs x =
              (if x \<in> dom (lookup_vdecls_ty vs) then
                Some (SOME v. \<exists>t. lookup_vdecls_ty vs x = Some t \<and> type_of_val A v = t)
-              else 
+              else
                None)"
 
-lemma named_state_var_context_dom: "dom (named_state_var_context A vs) = dom (lookup_vdecls_ty vs)" (is "dom (?f vs) = dom (?g vs)")  
+lemma named_state_var_context_dom: "dom (named_state_var_context A vs) = dom (lookup_vdecls_ty vs)" (is "dom (?f vs) = dom (?g vs)")
 proof
   show "dom (?f vs) \<subseteq> dom (?g vs)"
   proof
@@ -891,17 +891,17 @@ proof
       apply simp
       by (meson option.distinct(1))
   qed
-qed auto        
+qed auto
 
 fun extend_named_state_var_context :: "'a absval_ty_fun \<Rightarrow> vdecls \<Rightarrow> 'a named_state \<Rightarrow> 'a named_state"
-  where "extend_named_state_var_context A vs ns = 
+  where "extend_named_state_var_context A vs ns =
            named_state_var_context A vs ++ ns"
 
-lemma extend_named_state_var_context_dom: 
-  "dom (extend_named_state_var_context A vs ns) = dom ns \<union> dom (lookup_vdecls_ty vs)" 
+lemma extend_named_state_var_context_dom:
+  "dom (extend_named_state_var_context A vs ns) = dom ns \<union> dom (lookup_vdecls_ty vs)"
   by (simp add: named_state_var_context_dom)
 
-lemma named_state_var_context_state_typ_wf:  
+lemma named_state_var_context_state_typ_wf:
   assumes "list_all (closed \<circ> (fst \<circ> snd)) vs" and
          Inhabited: "\<And>t. closed t \<Longrightarrow> \<exists>v. type_of_val A v = t"
   shows "state_typ_wf A [] (named_state_var_context A vs) vs"
@@ -929,23 +929,23 @@ qed
 lemma extend_named_state_var_context_state_typ_wf:
   assumes Closed: "list_all (closed \<circ> (fst \<circ> snd)) vs" and
          Inhabited: "\<And>t. closed t \<Longrightarrow> \<exists>v. type_of_val A v = t" and
-         StateWellTy: "\<And>x t v. lookup_vdecls_ty vs x = Some t \<Longrightarrow> ns x = Some v \<Longrightarrow> 
-                      type_of_val A v = t"         
+         StateWellTy: "\<And>x t v. lookup_vdecls_ty vs x = Some t \<Longrightarrow> ns x = Some v \<Longrightarrow>
+                      type_of_val A v = t"
   shows "state_typ_wf A [] (extend_named_state_var_context A vs ns) vs"
   unfolding state_typ_wf_def
 proof (rule allI | rule impI)+
   fix x t
-  assume "lookup_vdecls_ty vs x = Some t"  
+  assume "lookup_vdecls_ty vs x = Some t"
 
   show "map_option (type_of_val A) (extend_named_state_var_context A vs ns x) = Some (instantiate [] t)"
-    
+
   proof (cases "x \<in> dom ns")
     case True
-    thus ?thesis 
-      using StateWellTy \<open>lookup_vdecls_ty vs x = Some t\<close> by auto      
+    thus ?thesis
+      using StateWellTy \<open>lookup_vdecls_ty vs x = Some t\<close> by auto
   next
     case False
-    then show ?thesis 
+    then show ?thesis
       using named_state_var_context_state_typ_wf[OF Closed Inhabited]
       by (metis \<open>lookup_vdecls_ty vs x = Some t\<close> extend_named_state_var_context.simps map_add_dom_app_simps(3) state_typ_wf_def)
   qed
@@ -956,20 +956,20 @@ subsection \<open>Constructing initial state\<close>
 subsubsection \<open>Global state\<close>
 
 fun initial_global_state_aux :: "program \<Rightarrow> tr_vpr_bpl \<Rightarrow> 'a full_total_state \<Rightarrow> ('a vbpl_absval) named_state"
-  where "initial_global_state_aux Pr Tr \<omega> x = 
+  where "initial_global_state_aux Pr Tr \<omega> x =
            (if x = heap_var Tr then
-              Some (AbsV (AHeap (construct_bpl_heap_from_vpr_heap Pr (field_translation Tr) (get_hh_total_full \<omega>))))
-           else 
+              Some (AbsV (AHeap (construct_bpl_heap_from_vpr_state Pr (field_translation Tr) (get_total_full \<omega>))))
+           else
              if x = mask_var Tr then
                 Some (AbsV (AMask (\<lambda>_. 0)))
-             else 
+             else
                 if x \<in> range (const_repr Tr) then
                   Some (boogie_const_val (SOME c. const_repr Tr c = x))
                 else
-                  (if (\<exists>f_vpr. declared_fields Pr f_vpr \<noteq> None \<and> field_translation Tr f_vpr = Some x)  then
-                    Some (AbsV (AField (NormalField x (SOME t. \<exists>f_vpr. field_translation Tr f_vpr = Some x \<and> 
+                  (if (\<exists>f_vpr. declared_fields Pr f_vpr \<noteq> None \<and> field_translation Tr f_vpr = Some x) then
+                    Some (AbsV (AField (NormalField x (SOME t. \<exists>f_vpr. field_translation Tr f_vpr = Some x \<and>
                                                                        declared_fields Pr f_vpr = Some t))))
-                   else None)             
+                   else None)
            )"
 
 lemma dom_initial_global_state_aux: "dom (initial_global_state_aux Pr Tr \<omega>) \<subseteq>
@@ -977,11 +977,11 @@ lemma dom_initial_global_state_aux: "dom (initial_global_state_aux Pr Tr \<omega
   unfolding dom_def ran_def
   by auto
 
-lemma initial_global_state_aux_heap: 
-  "initial_global_state_aux Pr Tr \<omega> (heap_var Tr) = Some (AbsV (AHeap (construct_bpl_heap_from_vpr_heap Pr (field_translation Tr) (get_hh_total_full \<omega>))))"
+lemma initial_global_state_aux_heap:
+  "initial_global_state_aux Pr Tr \<omega> (heap_var Tr) = Some (AbsV (AHeap (construct_bpl_heap_from_vpr_state Pr (field_translation Tr) (get_total_full \<omega>))))"
   by simp
 
-lemma initial_global_state_aux_mask: 
+lemma initial_global_state_aux_mask:
   assumes "disjoint_list [{heap_var Tr}, {mask_var Tr}, ran (field_translation Tr), range (const_repr Tr)]"
   shows  "initial_global_state_aux Pr Tr \<omega> (mask_var Tr) = Some (AbsV (AMask (\<lambda>_. 0)))"
 proof -
@@ -996,7 +996,7 @@ proof -
     by simp
 qed
 
-lemma initial_global_state_aux_const: 
+lemma initial_global_state_aux_const:
   assumes Disj: "disjoint_list [{heap_var Tr}, {mask_var Tr}, ran (field_translation Tr), range (const_repr Tr)]" and
           Const: "x \<in> range (const_repr Tr)"
         shows  "initial_global_state_aux Pr Tr \<omega> x = Some (boogie_const_val (SOME c. const_repr Tr c = x))"
@@ -1024,10 +1024,10 @@ proof -
     by simp
 qed
 
-lemma initial_global_state_aux_field: 
+lemma initial_global_state_aux_field:
   assumes Disj: "disjoint_list [{heap_var Tr}, {mask_var Tr}, ran (field_translation Tr), range (const_repr Tr)]" and
           Field: "\<exists>f_vpr. declared_fields Pr f_vpr \<noteq> None \<and> field_translation Tr f_vpr = Some x"
-  shows  "initial_global_state_aux Pr Tr \<omega> x = Some (AbsV (AField (NormalField x (SOME t. \<exists>f_vpr. field_translation Tr f_vpr = Some x \<and> 
+  shows  "initial_global_state_aux Pr Tr \<omega> x = Some (AbsV (AField (NormalField x (SOME t. \<exists>f_vpr. field_translation Tr f_vpr = Some x \<and>
                                                                        declared_fields Pr f_vpr = Some t))))"
 proof -
   have "x \<in> ran (field_translation Tr)"
@@ -1070,10 +1070,10 @@ qed
 lemma eq_someD:
   assumes "a = f (SOME t. Q t)" and "Q t"
   obtains t' where "Q t' \<and> a = f t'"
-  using assms 
+  using assms
   by (metis someI_ex)
 
-lemma initial_global_state_aux_field_2: 
+lemma initial_global_state_aux_field_2:
   assumes Disj: "disjoint_list [{heap_var Tr}, {mask_var Tr}, ran (field_translation Tr), range (const_repr Tr)]" and
           Inj: "inj_on (field_translation Tr) (dom (field_translation Tr))" and
           FieldTr: "field_translation Tr f_vpr = Some x" and
@@ -1084,38 +1084,38 @@ proof -
     using FieldTr FieldVpr
     by blast
 
-  note Aux = initial_global_state_aux_field[OF Disj *] 
+  note Aux = initial_global_state_aux_field[OF Disj *]
 
-  from FieldTr FieldVpr obtain f'_vpr t' where 
+  from FieldTr FieldVpr obtain f'_vpr t' where
     "?g x = Some (AbsV (AField (NormalField x t')))" and
-    "field_translation Tr f'_vpr = Some x \<and> declared_fields Pr f'_vpr = Some t'"  
+    "field_translation Tr f'_vpr = Some x \<and> declared_fields Pr f'_vpr = Some t'"
     using eq_someD[where ?f= "\<lambda>t. Some (AbsV (AField (NormalField x t)))", OF Aux]
     by metis
 
   thus ?thesis
-    using Inj FieldTr FieldVpr   
+    using Inj FieldTr FieldVpr
     by (metis domI inj_on_contraD option.inject)
 qed
 
-definition initial_global_state 
+definition initial_global_state
   where "initial_global_state T vs Pr Tr \<omega> \<equiv> extend_named_state_var_context (vbpl_absval_ty T) vs (initial_global_state_aux Pr Tr \<omega>)"
-                                                                                                              
+
 lemma initial_global_state_aux_typ_wf:
-  assumes 
+  assumes
           WfTyRepr: "wf_ty_repr_bpl T" and
           InjTrField:  "inj_on (field_translation Tr) (dom (field_translation Tr))" and
           Disj: "disjoint_list [{heap_var Tr}, {mask_var Tr}, ran (field_translation Tr), range (const_repr Tr)]" and
           Closed: "list_all (closed \<circ> (fst \<circ> snd)) vs" and
           VprHeapTy: "total_heap_well_typed Pr (domain_type T) (get_hh_total_full \<omega>)" and
           FieldTrTy: "\<And>f_vpr t_vpr. declared_fields Pr f_vpr = Some t_vpr \<Longrightarrow>
-                        \<exists>f_bpl t_bpl.  
+                        \<exists>f_bpl t_bpl.
                              field_translation Tr f_vpr = Some f_bpl \<and>
                              vpr_to_bpl_ty T t_vpr = Some t_bpl \<and>
                              lookup_vdecls_ty vs f_bpl = Some (TCon (TFieldId T) [TConSingle (TNormalFieldId T), t_bpl])" and
           HeapTy: "lookup_vdecls_ty vs (heap_var Tr) = Some (TConSingle (THeapId T))" and
           MaskTy: "lookup_vdecls_ty vs (mask_var Tr) = Some (TConSingle (TMaskId T))" and
           ConstTy: "\<And>c. lookup_vdecls_ty vs (const_repr Tr c) = Some (boogie_const_ty T c)"
-        shows "state_typ_wf (vbpl_absval_ty T) [] (initial_global_state T vs Pr Tr \<omega>) vs"
+    shows "state_typ_wf (vbpl_absval_ty T) [] (initial_global_state T vs Pr Tr \<omega>) vs"
   unfolding initial_global_state_def
 proof (rule extend_named_state_var_context_state_typ_wf[OF Closed closed_types_inhabited])
   let ?field_tr_dom = "{f_bpl. \<exists>f_vpr. declared_fields Pr f_vpr \<noteq> None \<and> field_translation Tr f_vpr = Some f_bpl}"
@@ -1131,61 +1131,61 @@ proof (rule extend_named_state_var_context_state_typ_wf[OF Closed closed_types_i
   show "type_of_vbpl_val T v = t"
   proof (cases rule: Set.UnE[OF *])
     case 1
-    then show ?thesis 
+    then show ?thesis
     proof (cases rule: Set.UnE[OF 1])
       case 1
       then show ?thesis
       proof (cases rule: Set.UnE[OF 1])
       case 1 \<comment>\<open>heap_var case\<close>
         hence "x = heap_var Tr" by simp
-        hence "v = (AbsV (AHeap (construct_bpl_heap_from_vpr_heap Pr (field_translation Tr) (get_hh_total_full \<omega>))))" (is "v = ?h")
+        hence "v = (AbsV (AHeap (construct_bpl_heap_from_vpr_state Pr (field_translation Tr) (get_total_full \<omega>))))" (is "v = ?h")
           using \<open>?ns x = Some v\<close>
           by simp
         have "type_of_vbpl_val T ?h = (TConSingle (THeapId T))"
-          using construct_bpl_heap_from_vpr_heap_correct_aux[OF WfTyRepr VprHeapTy _ InjTrField]
-          by simp      
-        
-        then show ?thesis        
-          using HeapTy LookupTy \<open>v = _\<close> \<open>x = heap_var Tr\<close> 
+          apply (simp only: vbpl_absval_ty.simps type_of_val.simps)
+          using construct_bpl_heap_from_vpr_state_correct_aux[OF WfTyRepr VprHeapTy[unfolded get_hh_total_full.simps] _ InjTrField, OF refl, unfolded Let_def, THEN conjunct2, THEN conjunct2, THEN conjunct2]
+          by auto
+        then show ?thesis
+          using HeapTy LookupTy \<open>v = _\<close> \<open>x = heap_var Tr\<close>
           by auto
       next
         case 2 \<comment>\<open>mask_var case\<close>
         hence "x = mask_var Tr" by simp
         hence "v = AbsV (AMask (\<lambda>_. 0))"
           using \<open>?ns x = Some v\<close>  initial_global_state_aux_mask[OF Disj, where ?Pr=Pr and ?\<omega>=\<omega>]
-          by simp        
-  
-        then show ?thesis 
+          by simp
+
+        then show ?thesis
           using MaskTy LookupTy \<open>x = _\<close>
-          by simp    
+          by simp
       qed
     next
       case 2 \<comment>\<open>field translation\<close>
-      from this obtain f_vpr t_vpr where FieldLookup: "declared_fields Pr f_vpr = Some t_vpr" and 
+      from this obtain f_vpr t_vpr where FieldLookup: "declared_fields Pr f_vpr = Some t_vpr" and
                                      FieldTr: "field_translation Tr f_vpr = Some x"
         by blast
-      from this obtain t_bpl where 
+      from this obtain t_bpl where
          TyBpl: "vpr_to_bpl_ty T t_vpr = Some t_bpl" and
-         LookupFieldTyBpl: "lookup_vdecls_ty vs x = Some (TCon (TFieldId T) [TConSingle (TNormalFieldId T), t_bpl])"         
+         LookupFieldTyBpl: "lookup_vdecls_ty vs x = Some (TCon (TFieldId T) [TConSingle (TNormalFieldId T), t_bpl])"
         using FieldTrTy[OF FieldLookup]
         by auto
-        
+
       from initial_global_state_aux_field_2[OF Disj InjTrField FieldTr FieldLookup, where ?\<omega>=\<omega>] have
          "v = AbsV (AField (NormalField x t_vpr))"
         using \<open>?ns x = Some v\<close>
         by simp
-        
+
       thus ?thesis
-        using LookupFieldTyBpl LookupTy TyBpl 
-        by simp        
+        using LookupFieldTyBpl LookupTy TyBpl
+        by simp
     qed
   next
     case 2 \<comment>\<open>const case\<close>
     hence "v = boogie_const_val (SOME c. const_repr Tr c = x)"
       using \<open>?ns x = Some v\<close> initial_global_state_aux_const[OF Disj \<open>x \<in> range (const_repr Tr)\<close>, where ?Pr = Pr and ?\<omega> = \<omega>]
-      by simp      
+      by simp
 
-    then show ?thesis 
+    then show ?thesis
       using boogie_const_val_well_ty ConstTy LookupTy
       by (metis (mono_tags, lifting) "2" image_iff option.inject verit_sko_ex')
   qed
@@ -1194,12 +1194,12 @@ qed
 subsubsection \<open>Local state\<close>
 
 fun initial_local_state_aux :: "tr_vpr_bpl \<Rightarrow> 'a full_total_state \<Rightarrow> ('a vbpl_absval) named_state"
-  where "initial_local_state_aux Tr \<omega> x = 
-           (if x \<in> ran (var_translation Tr) then 
-             Some (SOME v. \<exists>x_vpr v_vpr. var_translation Tr x_vpr = Some x \<and> 
-                                     get_store_total \<omega> x_vpr = Some v_vpr \<and> 
+  where "initial_local_state_aux Tr \<omega> x =
+           (if x \<in> ran (var_translation Tr) then
+             Some (SOME v. \<exists>x_vpr v_vpr. var_translation Tr x_vpr = Some x \<and>
+                                     get_store_total \<omega> x_vpr = Some v_vpr \<and>
                                      v = val_rel_vpr_bpl v_vpr)
-           else 
+           else
              None)"
 
 lemma dom_initial_local_state_aux: "dom (initial_local_state_aux Tr \<omega>) = ran (var_translation Tr)" (is "?A = ?B")
@@ -1225,8 +1225,8 @@ proof -
   from VarTrSome have "x_bpl \<in> ran (var_translation Tr)"
     by (simp add: ranI)
 
-  hence "?f x_bpl = Some (SOME v. \<exists>x_vpr v_vpr. var_translation Tr x_vpr = Some x_bpl \<and> 
-                                     get_store_total \<omega> x_vpr = Some v_vpr \<and> 
+  hence "?f x_bpl = Some (SOME v. \<exists>x_vpr v_vpr. var_translation Tr x_vpr = Some x_bpl \<and>
+                                     get_store_total \<omega> x_vpr = Some v_vpr \<and>
                                      v = val_rel_vpr_bpl v_vpr)" (is "_ = Some ?v")
     by simp
 
@@ -1235,7 +1235,7 @@ proof -
     "get_store_total \<omega> x_vpr' = Some v_vpr'"
     "?v = val_rel_vpr_bpl v_vpr'"
     using StoreSome VarTrSome
-    by (metis (no_types, lifting) calculation option.inject)    
+    by (metis (no_types, lifting) calculation option.inject)
 
   ultimately show ?thesis
     using assms
@@ -1247,11 +1247,11 @@ definition initial_local_state
   where "initial_local_state T vs Tr \<omega> \<equiv> extend_named_state_var_context (vbpl_absval_ty T) vs (initial_local_state_aux Tr \<omega>)"
 
 lemma initial_local_state_aux_typ_wf:
-  assumes 
+  assumes
           WfTyRepr: "wf_ty_repr_bpl T" and
           Closed: "list_all (closed \<circ> (fst \<circ> snd)) vs" and
           VarTranslationTy: "\<And> x_vpr x_bpl. var_translation Tr x_vpr = Some x_bpl \<Longrightarrow>
-                                   (\<exists>v_vpr. get_store_total \<omega> x_vpr = Some v_vpr \<and> 
+                                   (\<exists>v_vpr. get_store_total \<omega> x_vpr = Some v_vpr \<and>
                                             (\<exists>t. lookup_vdecls_ty vs x_bpl = Some t \<and>
                                                  type_of_vbpl_val T (val_rel_vpr_bpl v_vpr) = t))" and
           Inj:  "inj_on (var_translation Tr) (dom (var_translation Tr))"
@@ -1265,8 +1265,8 @@ proof (rule extend_named_state_var_context_state_typ_wf[OF Closed closed_types_i
   hence "x \<in> ran (var_translation Tr)"
     by (metis initial_local_state_aux.simps option.distinct(1))
 
-  hence "v = (SOME v. \<exists>x_vpr v_vpr. var_translation Tr x_vpr = Some x \<and> 
-                                     get_store_total \<omega> x_vpr = Some v_vpr \<and> 
+  hence "v = (SOME v. \<exists>x_vpr v_vpr. var_translation Tr x_vpr = Some x \<and>
+                                     get_store_total \<omega> x_vpr = Some v_vpr \<and>
                                      v = val_rel_vpr_bpl v_vpr)"
     using *
     by auto
@@ -1275,13 +1275,13 @@ proof (rule extend_named_state_var_context_state_typ_wf[OF Closed closed_types_i
     unfolding ran_def
     by blast
 
-  moreover from this obtain v_vpr where 
-        Store: "get_store_total \<omega> x_vpr = Some v_vpr" and 
+  moreover from this obtain v_vpr where
+        Store: "get_store_total \<omega> x_vpr = Some v_vpr" and
         TyBpl: "type_of_vbpl_val T (val_rel_vpr_bpl v_vpr) = t"
     using VarTranslationTy LookupTy
     by fastforce
 
-  have "\<exists>v x_vpr v_vpr. var_translation Tr x_vpr = Some x \<and> get_store_total \<omega> x_vpr = Some v_vpr \<and> 
+  have "\<exists>v x_vpr v_vpr. var_translation Tr x_vpr = Some x \<and> get_store_total \<omega> x_vpr = Some v_vpr \<and>
                                v = val_rel_vpr_bpl v_vpr"
     apply (rule exI)+
     apply (intro conjI)
@@ -1290,12 +1290,12 @@ proof (rule extend_named_state_var_context_state_typ_wf[OF Closed closed_types_i
     apply simp
     done
 
-  from this obtain x_vpr' v_vpr' where 
-    "var_translation Tr x_vpr' = Some x" and 
+  from this obtain x_vpr' v_vpr' where
+    "var_translation Tr x_vpr' = Some x" and
     "get_store_total \<omega> x_vpr' = Some v_vpr'" and
     "v = val_rel_vpr_bpl v_vpr'"
-    using \<open>v = _\<close>    
-    using * Inj initial_local_state_aux_Some 
+    using \<open>v = _\<close>
+    using * Inj initial_local_state_aux_Some
     by fastforce
 
   hence "v = val_rel_vpr_bpl v_vpr"
@@ -1320,7 +1320,7 @@ proof (induction rule: list_all2_induct)
   then show ?case by simp
 next
   case (Cons x xs y ys)
-  then show ?case 
+  then show ?case
   proof (cases "a = fst x")
     case True
     hence "map_of (y # ys) a = Some (snd y)"
@@ -1328,19 +1328,19 @@ next
     moreover from \<open>a = fst x\<close> have "snd x = b"
       using Cons
       by simp
-    ultimately show ?thesis 
+    ultimately show ?thesis
       using \<open>P x y\<close> \<open>a = fst x\<close>
       by (metis Fst prod.collapse)
   next
     case False
-    then show ?thesis 
-      using Cons Fst old.prod.exhaust 
+    then show ?thesis
+      using Cons Fst old.prod.exhaust
       by auto
-  qed   
+  qed
 qed
 
 definition field_tr_prop
-  where "field_tr_prop T global_decls f_vpr_ty_vpr f_vpr_f_bpl \<equiv>  
+  where "field_tr_prop T global_decls f_vpr_ty_vpr f_vpr_f_bpl \<equiv>
       \<exists>ty_bpl.
            (fst f_vpr_ty_vpr = fst f_vpr_f_bpl)   \<and>
             vpr_to_bpl_ty T (snd f_vpr_ty_vpr) = Some ty_bpl \<and>
@@ -1352,16 +1352,16 @@ lemma field_tr_prop_fst: "\<forall>f_vpr_ty_vpr f_vpr_f_bpl. field_tr_prop T glo
   by (simp add: field_tr_prop_def)
 
 definition var_rel_prop
-  where "var_rel_prop T local_decls ty_vpr var_vpr \<equiv> 
+  where "var_rel_prop T local_decls ty_vpr var_vpr \<equiv>
           \<exists>ty_bpl. vpr_to_bpl_ty T ty_vpr = Some ty_bpl \<and>
                    lookup_vdecls_ty local_decls var_vpr = Some ty_bpl"
 
 lemma var_rel_prop_aux:
-  assumes WellTy: "vpr_store_well_typed A \<Lambda> \<sigma>" 
+  assumes WellTy: "vpr_store_well_typed A \<Lambda> \<sigma>"
       and "domain_type T = A"
       and ListAll: "list_all (\<lambda>var_vpr_var_bpl. \<exists>t. \<Lambda> (fst var_vpr_var_bpl) = Some t \<and> var_rel_prop T local_decls t (snd var_vpr_var_bpl)) var_rel_list"
       and LookupVarRel: "map_of var_rel_list x_vpr = Some x_bpl"
-  shows "\<exists>v_vpr. \<sigma> x_vpr = Some v_vpr \<and> 
+  shows "\<exists>v_vpr. \<sigma> x_vpr = Some v_vpr \<and>
                                       (\<exists>t. lookup_vdecls_ty local_decls x_bpl = Some t \<and>
                                            type_of_vbpl_val T (val_rel_vpr_bpl v_vpr) = t)"
 proof -
@@ -1370,7 +1370,7 @@ proof -
            "var_rel_list ! i = (x_vpr, x_bpl)"
     by (meson in_set_conv_nth map_of_SomeD)
 
-  with ListAll 
+  with ListAll
   obtain t where "\<Lambda> x_vpr = Some t" and
            Prop: "var_rel_prop T local_decls t x_bpl"
     by (auto simp: list_all_length)
@@ -1385,7 +1385,7 @@ proof -
     unfolding var_rel_prop_def
     by blast
 qed
-    
+
 lemma boogie_const_rel_aux:
   assumes ConstTy: "\<And>c. lookup_vdecls_ty (fst \<Lambda>) (const_repr Tr c) = Some (boogie_const_ty T c)" and
           GlobalsLocalsDisj: "set (map fst (fst \<Lambda>)) \<inter> set (map fst (snd \<Lambda>)) = {}" and
@@ -1414,9 +1414,9 @@ lemma boogie_const_rel_aux:
   qed
 
 lemma field_rel_aux:
-assumes FieldTrTy: "\<And>f_vpr t_vpr. 
+assumes FieldTrTy: "\<And>f_vpr t_vpr.
                               declared_fields Pr f_vpr = Some t_vpr \<Longrightarrow>
-                            \<exists> f_bpl.  
+                            \<exists> f_bpl.
                                field_translation Tr f_vpr = Some f_bpl \<and>
                                field_tr_prop T (fst \<Lambda>) (f_vpr, t_vpr) (f_vpr, f_bpl)"
     and GlobalsLocalsDisj: "set (map fst (fst \<Lambda>)) \<inter> set (map fst (snd \<Lambda>)) = {}"
@@ -1439,15 +1439,15 @@ assumes FieldTrTy: "\<And>f_vpr t_vpr.
       unfolding ran_def
       by blast
 
-    from FieldGlobal GlobalsLocalsDisj have 
+    from FieldGlobal GlobalsLocalsDisj have
       "lookup_var \<Lambda> ns f_bpl = global_state ns f_bpl"
       by (metis lookup_var_global_disj lookup_vdecls_ty_map_of prod.exhaust_sel)
-    
+
     moreover from initial_global_state_aux_field_2[OF DisjAux InjFieldTr FieldTr FieldLookup, where ?\<omega>=\<omega>]
     have "global_state ns f_bpl = Some (AbsV (AField (NormalField f_bpl t_vpr)))"
       using InitGlobalState \<open>f_bpl \<in> _\<close>
       by (simp add: initial_global_state_def)
-    
+
     ultimately show "has_Some (\<lambda>f_bpl. lookup_var \<Lambda> ns f_bpl = Some (AbsV (AField (NormalField f_bpl t_vpr)))) (field_translation Tr f_vpr)"
       using FieldTr
       by simp
@@ -1455,30 +1455,30 @@ assumes FieldTrTy: "\<And>f_vpr t_vpr.
 
 definition disj_vars_state_relation
   where "disj_vars_state_relation Tr AuxPred =
-              disjoint_list [{heap_var Tr, heap_var_def Tr}, {mask_var Tr, mask_var_def Tr}, ran (var_translation Tr), 
+              disjoint_list [{heap_var Tr, heap_var_def Tr}, {mask_var Tr, mask_var_def Tr}, ran (var_translation Tr),
                                ran (field_translation Tr), range (const_repr Tr), dom AuxPred]"
 
 definition field_tr_prop_full
-  where "field_tr_prop_full Pr global_vdecls TyRep FieldTr \<equiv> \<forall>f_vpr t_vpr. 
+  where "field_tr_prop_full Pr global_vdecls TyRep FieldTr \<equiv> \<forall>f_vpr t_vpr.
                           declared_fields Pr f_vpr = Some t_vpr \<longrightarrow>
-                          (\<exists> f_bpl.  
+                          (\<exists> f_bpl.
                            FieldTr f_vpr = Some f_bpl \<and>
                            field_tr_prop TyRep global_vdecls (f_vpr, t_vpr) (f_vpr, f_bpl))"
 
 lemma init_state_in_state_relation:
-  assumes  WfTyRepr: "wf_ty_repr_bpl T" and
-         Disj: "disj_vars_state_relation Tr Map.empty" and
+  assumes WfTyRepr: "wf_ty_repr_bpl T" and
+          Disj: "disj_vars_state_relation Tr Map.empty" and
           "is_empty_total_full \<omega>" and
           ViperHeapWellTy: "total_heap_well_typed ((program_total ctxt_vpr)) (absval_interp_total ctxt_vpr) (get_hh_total_full \<omega>)" and
           WfMask: "wf_mask_simple (get_mh_total_full \<omega>)" and
           Consistent: "StateCons \<omega> \<and> consistent_external (total_context.make (program_total ctxt_vpr) (\<lambda>_. None) (domain_type T)) (get_total_full \<omega>)" and
-         TyInterp: "type_interp ctxt = vbpl_absval_ty T" and
+          TyInterp: "type_interp ctxt = vbpl_absval_ty T" and
           DomainTy:  "domain_type T = absval_interp_total ctxt_vpr" and
           "ns = \<lparr> old_global_state = initial_global_state T (fst (var_context ctxt)) (program_total ctxt_vpr) Tr \<omega>,
                   global_state = initial_global_state T (fst (var_context ctxt)) (program_total ctxt_vpr) Tr \<omega>,
                   local_state = initial_local_state T (snd (var_context ctxt)) Tr \<omega>,
                   binder_state = Map.empty \<rparr>" and
-         InjVarTr: "inj_on (var_translation Tr) (dom (var_translation Tr))" and
+          InjVarTr: "inj_on (var_translation Tr) (dom (var_translation Tr))" and
 
           ClosedGlobals: "list_all (closed \<circ> (fst \<circ> snd)) (fst (var_context ctxt))" and
           ClosedLocals: "list_all (closed \<circ> (fst \<circ> snd)) (snd (var_context ctxt))" and
@@ -1497,7 +1497,7 @@ lemma init_state_in_state_relation:
 
 \<comment>\<open>Local state assumptions\<close>
           VarTranslationTy: "\<And> x_vpr x_bpl. var_translation Tr x_vpr = Some x_bpl \<Longrightarrow>
-                                   (\<exists>v_vpr. get_store_total \<omega> x_vpr = Some v_vpr \<and> 
+                                   (\<exists>v_vpr. get_store_total \<omega> x_vpr = Some v_vpr \<and>
                                             (\<exists>t. lookup_vdecls_ty (snd (var_context ctxt)) x_bpl = Some t \<and>
                                                  type_of_vbpl_val T (val_rel_vpr_bpl v_vpr) = t))"
 
@@ -1514,7 +1514,7 @@ proof -
   note DisjSimp = Disj[simplified disj_vars_state_relation_def]
 
   have "disjoint_list [{heap_var Tr, heap_var_def Tr}, {mask_var Tr, mask_var_def Tr}, ran (field_translation Tr), range (const_repr Tr)]"
-    by (rule disjoint_list_sublist[OF DisjSimp]) fastforce    
+    by (rule disjoint_list_sublist[OF DisjSimp]) fastforce
   hence DisjAux: "disjoint_list [{heap_var Tr}, {mask_var Tr}, ran (field_translation Tr), range (const_repr Tr)]"
     by (rule disjoint_list_subset_list_all2) blast
 
@@ -1523,42 +1523,42 @@ proof -
   proof (rule conjI[OF \<open>is_empty_total_full \<omega>\<close>], intro conjI)
 
     have Aux: "\<And>var_vpr var_bpl val_vpr.
-         var_translation Tr var_vpr = Some var_bpl \<Longrightarrow> get_store_total \<omega> var_vpr = Some val_vpr \<Longrightarrow> 
+         var_translation Tr var_vpr = Some var_bpl \<Longrightarrow> get_store_total \<omega> var_vpr = Some val_vpr \<Longrightarrow>
          lookup_var (var_context ctxt) ns var_bpl = Some (val_rel_vpr_bpl val_vpr)"
-    proof -    
+    proof -
       fix var_vpr var_bpl val_vpr
       assume VarTrSome: "var_translation Tr var_vpr = Some var_bpl" and
-             "get_store_total \<omega> var_vpr = Some val_vpr" 
-  
+             "get_store_total \<omega> var_vpr = Some val_vpr"
+
       moreover from this obtain t where LookupTy: "lookup_vdecls_ty (snd (var_context ctxt)) var_bpl = Some t"
         using VarTranslationTy
         by blast
-  
+
       ultimately have "local_state ns var_bpl = Some (val_rel_vpr_bpl val_vpr)"
         apply (subst \<open>local_state ns = _\<close>)
         using initial_local_state_aux_Some[OF InjVarTr]
         by (fastforce simp: initial_local_state_def)
-  
+
       thus "lookup_var (var_context ctxt) ns var_bpl = Some (val_rel_vpr_bpl val_vpr)"
         using LookupTy
         by (metis lookup_var_local lookup_vdecls_ty_map_of prod.exhaust_sel)
     qed
-             
+
     show "store_rel (type_interp ctxt) (var_context ctxt) (var_translation Tr) \<omega> ns"
       unfolding store_rel_def
       apply (rule conjI[OF InjVarTr], (rule allI | rule impI)+)
       using VarTranslationTy TyInterp Aux
       by (metis lookup_vdecls_ty_local_3)
-  
+
   next
-  
+
     show "heap_var_rel (program_total ctxt_vpr) (var_context ctxt) T (field_translation Tr) (heap_var Tr) \<omega> ns"
       unfolding heap_var_rel_def
     proof (intro conjI, rule exI, intro conjI)
-      have "global_state ns (heap_var Tr) = Some (AbsV (AHeap (construct_bpl_heap_from_vpr_heap (program_total ctxt_vpr) (field_translation Tr) (get_hh_total_full \<omega>))))"
+      have "global_state ns (heap_var Tr) = Some (AbsV (AHeap (construct_bpl_heap_from_vpr_state (program_total ctxt_vpr) (field_translation Tr) (get_total_full \<omega>))))"
                       (is "_ = Some (AbsV (AHeap ?hb))")
-        by (simp add: \<open>global_state ns = _\<close> initial_global_state_def) 
-    
+        by (simp add: \<open>global_state ns = _\<close> initial_global_state_def)
+
       with GlobalsLocalsDisj and HeapTy
       show "lookup_var (var_context ctxt) ns (heap_var Tr) = Some (AbsV (AHeap ?hb))"
         by (metis lookup_var_global_disj lookup_vdecls_ty_map_of prod.collapse)
@@ -1567,51 +1567,61 @@ proof -
       show "lookup_var_ty (var_context ctxt) (heap_var Tr) = Some (TConSingle (THeapId T))"
         by (metis lookup_var_decl_global_2 lookup_var_ty_def lookup_vdecls_ty_def lookup_vdecls_ty_map_of)
     next
-      show "vbpl_absval_ty_opt T (AHeap (construct_bpl_heap_from_vpr_heap (program_total ctxt_vpr) (field_translation Tr) (get_hh_total_full \<omega>))) = Some (THeapId T, [])"
-        using construct_bpl_heap_from_vpr_heap_correct_aux[OF WfTyRepr ViperHeapWellTy DomainTy InjFieldTr] 
+      show "vbpl_absval_ty_opt T (AHeap (construct_bpl_heap_from_vpr_state (program_total ctxt_vpr) (field_translation Tr) (get_total_full \<omega>))) = Some (THeapId T, [])"
+        using construct_bpl_heap_from_vpr_state_correct_aux[OF WfTyRepr ViperHeapWellTy[unfolded get_hh_total_full.simps] DomainTy InjFieldTr]
         by meson
     next
       show "heap_rel (program_total ctxt_vpr) (field_translation Tr) (get_hh_total_full \<omega>)
-       (construct_bpl_heap_from_vpr_heap (program_total ctxt_vpr) (field_translation Tr) (get_hh_total_full \<omega>))"
-        using construct_bpl_heap_from_vpr_heap_correct_aux[OF WfTyRepr ViperHeapWellTy DomainTy InjFieldTr] 
-        by meson
-    next 
-      show "total_heap_well_typed (program_total ctxt_vpr) (domain_type T) (get_hh_total_full \<omega>)"        
+       (construct_bpl_heap_from_vpr_state (program_total ctxt_vpr) (field_translation Tr) (get_total_full \<omega>))"
+        using construct_bpl_heap_from_vpr_state_correct_aux[OF WfTyRepr ViperHeapWellTy[unfolded get_hh_total_full.simps] DomainTy InjFieldTr]
+        by (metis get_hh_total_full.simps)
+    next
+      show "total_heap_well_typed (program_total ctxt_vpr) (domain_type T) (get_hh_total_full \<omega>)"
         using DomainTy ViperHeapWellTy by auto
     qed
-  
+
     thus "heap_var_rel (program_total ctxt_vpr) (var_context ctxt) T (field_translation Tr) (heap_var_def Tr) \<omega> ns"
       using \<open>heap_var Tr = _\<close>
       by simp
-  next  
+  next
     show "mask_var_rel (program_total ctxt_vpr) (var_context ctxt) T (field_translation Tr) (mask_var Tr) \<omega> ns"
       unfolding mask_var_rel_def
     proof (rule exI, intro conjI)
-                    
+
       have "global_state ns (mask_var Tr) = Some (AbsV (AMask zero_mask_bpl))"
                       (is "_ = Some (AbsV (AMask ?mb))")
         apply (subst \<open>global_state ns = _\<close>)
         using initial_global_state_aux_mask[OF DisjAux, where ?Pr="program_total ctxt_vpr" and ?\<omega>=\<omega>]
         by (simp add: initial_global_state_def)
-  
-      with GlobalsLocalsDisj and MaskTy      
+
+      with GlobalsLocalsDisj and MaskTy
       show "lookup_var (var_context ctxt) ns (mask_var Tr) = Some (AbsV (AMask ?mb))"
         by (metis lookup_var_global_disj lookup_vdecls_ty_map_of prod.collapse)
     next
       show "lookup_var_ty (var_context ctxt) (mask_var Tr) = Some (TConSingle (TMaskId T))"
         using GlobalsLocalsDisj and MaskTy
         by (metis (no_types, opaque_lifting) lookup_var_decl_global_2 lookup_var_ty_def lookup_vdecls_ty_def lookup_vdecls_ty_map_of option.inject)
-    next    
+    next
       show "mask_rel (program_total ctxt_vpr) (field_translation Tr) (get_mh_total_full \<omega>) (get_mp_total_full \<omega>) zero_mask_bpl"
         using \<open>is_empty_total_full \<omega>\<close>
         unfolding mask_rel_def is_empty_total_full_def is_empty_total_def zero_mask_def zero_nested_mask_def
         by (simp add: zero_preal.rep_eq)
     qed
-  
+
     thus "mask_var_rel (program_total ctxt_vpr) (var_context ctxt) T (field_translation Tr) (mask_var_def Tr) \<omega> ns"
       using \<open>mask_var Tr = _\<close>
       by simp
-  
+
+  next
+    have "global_state ns (heap_var Tr) = Some (AbsV (AHeap (construct_bpl_heap_from_vpr_state (program_total ctxt_vpr) (field_translation Tr) (get_total_full \<omega>))))"
+                    (is "_ = Some (AbsV (AHeap ?hb))")
+      by (simp add: \<open>global_state ns = _\<close> initial_global_state_def)
+    thus "heap_knownfolded_var_rel (knownfolded_state_rel_opt (state_rel_opt Tr))
+            (program_total ctxt_vpr) (var_context ctxt) (field_translation Tr) (heap_var Tr) \<omega> ns"
+      unfolding heap_knownfolded_var_rel_def heap_knownfolded_rel_def \<open>ns = _\<close> initial_global_state_def
+      by (metis (no_types, lifting) GlobalsLocalsDisj HeapTy Semantics.val.inject(2) construct_bpl_heap_from_vpr_heap_aux_2 lookup_var_global_disj lookup_vdecls_ty_map_of prod.collapse vb_field.simps(8) vbpl_absval.inject(6))
+
+  next
     show "field_rel (program_total ctxt_vpr) (var_context ctxt) (field_translation Tr) ns"
       unfolding field_rel_def
     proof (rule conjI[OF InjFieldTr], (rule allI | rule impI)+)
@@ -1624,25 +1634,25 @@ proof -
         unfolding field_tr_prop_full_def field_tr_prop_def
         by fastforce
 
-      from FieldGlobal GlobalsLocalsDisj have 
+      from FieldGlobal GlobalsLocalsDisj have
         "lookup_var (var_context ctxt) ns f_bpl = global_state ns f_bpl"
         by (metis lookup_var_global_disj lookup_vdecls_ty_map_of prod.exhaust_sel)
-      
+
       moreover from initial_global_state_aux_field_2[OF DisjAux InjFieldTr FieldTr FieldLookup, where ?\<omega>=\<omega>]
       have "global_state ns f_bpl = Some (AbsV (AField (NormalField f_bpl t_vpr)))"
         using \<open>global_state ns = _\<close>
         by (simp add: initial_global_state_def)
-      
+
       ultimately show "has_Some (\<lambda>f_bpl. lookup_var (var_context ctxt) ns f_bpl = Some (AbsV (AField (NormalField f_bpl t_vpr)))) (field_translation Tr f_vpr)"
         using FieldTr
         by simp
     qed
-  next  
+  next
     show "boogie_const_rel (const_repr Tr) (var_context ctxt) ns"
       using ConstTy GlobalsLocalsDisj DisjAux \<open>global_state ns = _\<close> InjConstRepr boogie_const_rel_aux
       by metis
   next
-  
+
     show "state_well_typed (type_interp ctxt) (var_context ctxt) [] ns"
       unfolding state_well_typed_def
     proof (intro conjI)
@@ -1660,7 +1670,7 @@ proof -
         using FieldTrTy
         unfolding field_tr_prop_full_def field_tr_prop_def
         by simp
-    
+
       thus "state_typ_wf (type_interp ctxt) [] (old_global_state ns) (fst (var_context ctxt))"
         using \<open>old_global_state ns = _\<close>
         by simp
@@ -1668,7 +1678,7 @@ proof -
       show "binder_state ns = Map.empty"
         by (rule \<open>binder_state ns = _\<close>)
     qed
-  next  
+  next
     show "aux_vars_pred_sat (var_context ctxt) Map.empty ns"
       by (simp add: aux_vars_pred_sat_def)
   qed (insert assms DisjSimp, auto)
@@ -1687,7 +1697,7 @@ proof
     using RanFieldTr
     unfolding ran_def
     by blast
-  with DomEq 
+  with DomEq
   show "\<exists>f_vpr. declared_fields Pr f_vpr \<noteq> None \<and> field_translation Tr f_vpr = Some c"
     by blast
 qed
@@ -1702,14 +1712,14 @@ proof (induction unique_cs)
   case Nil
   then show ?case by (simp add: unique_constants_distinct_def)
 next
-  case (Cons c cs)  
+  case (Cons c cs)
 
   have GlobalStateFieldLookup: "\<And> c'. c' \<in> set (c#cs) \<Longrightarrow> \<exists>t. ?gs c' = Some (AbsV (AField (NormalField c' t)))"
   proof -
     fix c'
     assume "c' \<in> set (c#cs)"
-    from this Cons obtain f_vpr where FieldLookup: "declared_fields Pr f_vpr \<noteq> None" and 
-                               FieldTr: "field_translation Tr f_vpr = Some c'"    
+    from this Cons obtain f_vpr where FieldLookup: "declared_fields Pr f_vpr \<noteq> None" and
+                               FieldTr: "field_translation Tr f_vpr = Some c'"
       by fast
 
     with initial_global_state_aux_field[OF Disj]
@@ -1720,10 +1730,10 @@ next
       by simp
     thus "\<exists>t. ?gs c' = Some (AbsV (AField (NormalField c' t)))"
       by simp
-  qed 
+  qed
 
-  show ?case 
-    unfolding unique_constants_distinct_def 
+  show ?case
+    unfolding unique_constants_distinct_def
   proof (simp, rule conjI)
     show "distinct (map (\<lambda>x. the (?gs x)) cs)"
     proof -
@@ -1737,9 +1747,9 @@ next
 
   next
     show "the (?gs c) \<notin> (\<lambda>x. the (?gs x)) ` set cs" (is "_ \<notin> ?M")
-    proof 
+    proof
       assume "the (?gs c) \<in> ?M"
-      from this obtain c' where 
+      from this obtain c' where
         "c' \<in> set cs" and
         Eq: "the (?gs c) = the (?gs c')"
         by blast
@@ -1770,11 +1780,11 @@ lemma inter_disjoint_intervals:
           "\<forall>x \<in> B. x \<ge> b_min \<and> x \<le> b_max" and
           "a_min \<le> a_max \<and> b_min \<le> b_max \<and> (a_max < b_min \<or> b_max < a_min)"
         shows "A \<inter> B = {}"
-  using assms  
-  by fastforce     
+  using assms
+  by fastforce
 
-method rename_case_simp_tac = 
-     (rename_tac j1, 
+method rename_case_simp_tac =
+     (rename_tac j1,
       case_tac j1,
       solves \<open>simp add: Set.Int_commute\<close>)
 
@@ -1787,7 +1797,7 @@ lemma disj_helper_tr_vpr_bpl:
           "ran (var_translation Tr) \<inter> range (const_repr Tr) = {}" and
           "ran (field_translation Tr) \<inter> range (const_repr Tr) = {}"
 
-  shows "disjoint_list [{heap_var Tr}, {mask_var Tr}, ran (var_translation Tr), 
+  shows "disjoint_list [{heap_var Tr}, {mask_var Tr}, ran (var_translation Tr),
                                ran (field_translation Tr), range (const_repr Tr)]" (is "disjoint_list ?M")
   unfolding disjoint_list_def
 proof clarify
@@ -1796,7 +1806,7 @@ proof clarify
          "i < length ?M" and
          "0 \<le> j" and
          "j < length ?M" and
-         "i \<noteq> j" 
+         "i \<noteq> j"
   thus  "disjnt (?M ! i) (?M ! j)"
     unfolding disjnt_def
     apply (cases i)
@@ -1804,7 +1814,7 @@ proof clarify
      \<comment>\<open> i = 0 \<close>
 
      apply (cases j)
-      apply simp 
+      apply simp
       apply (solves \<open>simp\<close> | rename_case_simp_tac)+
     apply (rename_tac i1)
     apply (case_tac i1)
@@ -1849,7 +1859,7 @@ proof clarify
   show "disjnt ((xs @ [{}]) ! i) ((xs @ [{}]) ! j)"
   proof (cases "i = length xs \<or> j = length xs")
     case True
-    then show ?thesis 
+    then show ?thesis
       using *
       unfolding disjnt_def
       by fastforce
@@ -1857,10 +1867,10 @@ proof clarify
     case False
     with * have "i < length xs \<and> j < length xs"
       by simp
-    then show ?thesis 
+    then show ?thesis
       using assms *
       unfolding disjoint_list_def
-      by (metis list_update_append1 list_update_id nth_list_update_eq)            
+      by (metis list_update_append1 list_update_id nth_list_update_eq)
   qed
 qed
 
@@ -1869,7 +1879,7 @@ lemma disjoint_list_drop_last:
      and "xs = xs'@[x]" \<comment>\<open>add as separate assumption such conclusion unifies with more goals\<close>
    shows "disjoint_list xs'"
   apply (rule disjoint_list_sublist[OF assms(1)])
-  using assms  
+  using assms
   by force
 
 lemma disjoint_list_drop_i:
@@ -1877,8 +1887,8 @@ lemma disjoint_list_drop_i:
       and "i < length xs"
       and "xs' = take i xs @ drop (i+1) xs"
     shows "disjoint_list (xs' :: ('a set) list)"
-proof - 
-  from \<open>i < length xs\<close> 
+proof -
+  from \<open>i < length xs\<close>
   have "xs = take i xs @ ((xs ! i) # drop (i+1) xs)"
     by (simp add: id_take_nth_drop)
 
@@ -1912,8 +1922,8 @@ method disjoint_globals_aux_tac uses disj_prop_aux =
 
 lemma initial_global_state_state_restriction:
   assumes Disj: "disjoint_list [{heap_var Tr}, {mask_var Tr}, ran (field_translation Tr), range (const_repr Tr)]" and
-          ConstantsRange:"set (map fst constants) = range (const_repr Tr) \<union> ran (field_translation Tr)" and 
-          Elem: "x \<in> range (const_repr Tr) \<union> ran (field_translation Tr)" 
+          ConstantsRange:"set (map fst constants) = range (const_repr Tr) \<union> ran (field_translation Tr)" and
+          Elem: "x \<in> range (const_repr Tr) \<union> ran (field_translation Tr)"
   shows "state_restriction (initial_global_state T (constants@globals) Pr Tr \<omega>) constants x = initial_global_state T constants Pr Tr \<omega> x"
   unfolding state_restriction_def
 proof -
@@ -1926,7 +1936,7 @@ proof -
   have "?ns0 x = ?ns1 x"
   proof (cases rule:  Set.UnE[OF \<open>x \<in> _\<close>])
     case 1
-    show ?thesis 
+    show ?thesis
       apply (simp add: initial_global_state_def, rule Aux)
       using initial_global_state_aux_const[OF Disj 1]
       by blast
@@ -1935,7 +1945,7 @@ proof -
     show ?thesis
     proof (cases "\<exists>f_vpr. declared_fields Pr f_vpr \<noteq> None \<and> field_translation Tr f_vpr = Some x")
       case True
-      show ?thesis         
+      show ?thesis
         apply (simp add: initial_global_state_def, rule Aux)
         using initial_global_state_aux_field[OF Disj True]
         by blast
@@ -1975,23 +1985,23 @@ proof -
       from \<open>x \<in> set (map fst constants)\<close> have
           DomConstantsGlobals: "x \<in> dom (lookup_vdecls_ty (constants@globals))"
         unfolding lookup_vdecls_ty_def
-        using DomConstants lookup_vdecls_ty_def by force       
-        
-      have "named_state_var_context (vbpl_absval_ty T) constants x = 
+        using DomConstants lookup_vdecls_ty_def by force
+
+      have "named_state_var_context (vbpl_absval_ty T) constants x =
            Some (SOME v. \<exists>t. lookup_vdecls_ty constants x = Some t \<and> type_of_val (vbpl_absval_ty T) v = t)"
         using ConstantsRange Elem
         by (simp add: DomConstants)
 
       have "lookup_vdecls_ty constants x = lookup_vdecls_ty (constants@globals) x"
         using lookup_vdecls_ty_def DomConstants
-        by auto         
+        by auto
       hence "named_state_var_context (vbpl_absval_ty T) constants x = named_state_var_context (vbpl_absval_ty T) (constants@globals) x"
         using DomConstants DomConstantsGlobals
         by simp
-      with LookupAux show ?thesis 
+      with LookupAux show ?thesis
         unfolding initial_global_state_def
         by (simp add: domIff map_add_dom_app_simps(3))
-    qed     
+    qed
   qed
 
   moreover have "map_of constants x \<noteq> None"
@@ -1999,25 +2009,25 @@ proof -
     by (simp add: map_of_eq_None_iff)
 
   ultimately show "option_if (map_of constants x \<noteq> None) (?ns0 x) = ?ns1 x"
-    by presburger  
+    by presburger
 qed
 
 lemma boogie_axioms_state_restriction_aux:
   assumes "gs = initial_global_state T (constants@globals) Pr Tr \<omega>" and
           "C = const_repr Tr" and
-         ConstTy: "\<And>c. lookup_vdecls_ty constants (const_repr Tr c) = Some (boogie_const_ty T c)" and 
+         ConstTy: "\<And>c. lookup_vdecls_ty constants (const_repr Tr c) = Some (boogie_const_ty T c)" and
          FieldProp: "field_tr_prop_full Pr constants T (field_translation Tr)" and
-          Disj: "disjoint_list [{heap_var Tr}, {mask_var Tr}, ran (field_translation Tr), range (const_repr Tr)]" and          
+          Disj: "disjoint_list [{heap_var Tr}, {mask_var Tr}, ran (field_translation Tr), range (const_repr Tr)]" and
           InjConstRepr: "inj (const_repr Tr)" and
           InjFieldTr: "inj_on (field_translation Tr) (dom (field_translation Tr))" and
-          ConstantsRange:"set (map fst constants) = range (const_repr Tr) \<union> ran (field_translation Tr)" and 
-         AxiomsSatGeneral: "\<And> ns. boogie_const_rel C (constants, []) ns \<Longrightarrow>  
+          ConstantsRange:"set (map fst constants) = range (const_repr Tr) \<union> ran (field_translation Tr)" and
+         AxiomsSatGeneral: "\<And> ns. boogie_const_rel C (constants, []) ns \<Longrightarrow>
                                   field_rel Pr (constants, []) (field_translation Tr) ns \<Longrightarrow>
                                   axioms_sat A (constants, []) \<Gamma> ns axioms"
   shows "axioms_sat A (constants, []) \<Gamma> (global_to_nstate (state_restriction gs constants)) axioms"
 proof -
   let ?ns = "(global_to_nstate (state_restriction gs constants))"
-  have "boogie_const_rel (const_repr Tr) (constants, []) ?ns"    
+  have "boogie_const_rel (const_repr Tr) (constants, []) ?ns"
     apply (rule boogie_const_rel_aux)
         apply (simp add: ConstTy)
        apply simp
@@ -2045,7 +2055,7 @@ proof -
     by simp
 qed
 
-lemma expr_sat_rewrite: "\<lbrakk>A,\<Lambda>,\<Gamma>,\<Omega> \<turnstile> \<langle>e,ns\<rangle> \<Down> LitV (LBool b); b\<rbrakk> \<Longrightarrow> A,\<Lambda>,\<Gamma>,\<Omega> \<turnstile> \<langle>e,ns\<rangle> \<Down> LitV (LBool True)"  
+lemma expr_sat_rewrite: "\<lbrakk>A,\<Lambda>,\<Gamma>,\<Omega> \<turnstile> \<langle>e,ns\<rangle> \<Down> LitV (LBool b); b\<rbrakk> \<Longrightarrow> A,\<Lambda>,\<Gamma>,\<Omega> \<turnstile> \<langle>e,ns\<rangle> \<Down> LitV (LBool True)"
   by simp
 
 lemma heap_upd_ty_preserved_2:
@@ -2066,11 +2076,11 @@ proof -
   moreover from type_of_val_not_dummy[OF FieldTy2]
   have "field_ty_fun_opt T f = Some (TFieldId T, [\<tau>, \<tau>'])"
     by simp
-    
+
   ultimately show ?thesis
     using heap_upd_ty_preserved NewVal
     by (metis OldHeap type_of_val.simps(2) vbpl_absval_ty.simps)
-qed   
+qed
 
 lemma heap_upd_ty_preserved_2_concrete:
   assumes wf_ty_repr: "wf_ty_repr_bpl (ty_repr_basic A\<lparr> pred_snap_field_type := PredFieldType \<rparr>)"
